added map to stack example - still missing table instantiation

theories/stack.v
@@ -14,107 +14,19 @@ Unset Printing Implicit Defensive.
 
 Close Scope byte_scope.
 
-Let expr := iris_use.expr.
-Let val := iris_use.val.
-Let to_val := iris_use.to_val.
+
+Notation "{{{ P }}} es {{{ v , Q }}}" :=
+  (□ ∀ Φ, P -∗ (∀ v : iris.val, Q -∗ Φ v) -∗ WP (es : iris.expr) @ NotStuck ; ⊤ {{ v, Φ v }})%I (at level 50). 
+   
 
 
 Section stack.
-  
-  Import DummyHosts.
-  Import uPred.
-  (*
-Variable host_function : eqType.
 
 
-Let host := host.host host_function.
-Let function_closure := function_closure host_function.
-Let store_record := store_record host_function.
-
-
-Variable host_instance : host.
-*)
-
-Let reduce := @reduce host_function host_instance.
-
-(*
-Let wasm_mixin : LanguageMixin _ _ _ := wasm_mixin host_instance.
- *)
 Canonical Structure wasm_lang := Language wasm_mixin.
 
-(* Let reducible := @reducible wasm_lang. *)
-(* Context `{!wfuncG Σ, !wtabG Σ, !wtabsizeG Σ, !wmemG Σ, !wmemsizeG Σ, !wglobG Σ, !wframeG Σ, !hvisG Σ, !hmsG Σ,  !logrel_na_invs Σ}. *)
  Context `{!wfuncG Σ, !wtabG Σ, !wtabsizeG Σ, !wmemG Σ, !wmemsizeG Σ, !wglobG Σ, !wframeG Σ, !wtablimitG Σ, !wmemlimitG Σ}. 
-(*
-(* TODO: Resolve duplicated notations *)
-Notation "n ↦[wf]{ q } v" := (mapsto (L:=N) (V:=function_closure) n q v%V)
-                           (at level 20, q at level 5, format "n ↦[wf]{ q } v") : bi_scope.
-Notation "n ↦[wf] v" := (mapsto (L:=N) (V:=function_closure) n (DfracOwn 1) v%V)
-                      (at level 20, format "n ↦[wf] v") : bi_scope.
-Notation "n ↦[wt]{ q } [ i ] v" := (mapsto (L:=N*N) (V:=funcelem) (n, i) q v%V)
-                           (at level 20, q at level 5, format "n ↦[wt]{ q } [ i ] v") : bi_scope.
-Notation "n ↦[wt][ i ] v" := (mapsto (L:=N*N) (V:=funcelem) (n, i) (DfracOwn 1) v%V)
-                      (at level 20, format "n ↦[wt][ i ] v") : bi_scope.
-Notation "n ↦[wm]{ q } [ i ] v" := (mapsto (L:=N*N) (V:=byte) (n, i) q v%V)
-                           (at level 20, q at level 5, format "n ↦[wm]{ q } [ i ] v") : bi_scope.
-Notation "n ↦[wm][ i ] v" := (mapsto (L:=N*N) (V:=byte) (n, i) (DfracOwn 1) v% V)
-                           (at level 20, format "n ↦[wm][ i ] v") : bi_scope.
-Notation "n ↦[wmlength] v" := (mapsto (L:=N) (V:=N) n (DfracOwn 1) v% V)
-                           (at level 20, format "n ↦[wmlength] v") : bi_scope.
-Notation "n ↦[wg]{ q } v" := (mapsto (L:=N) (V:=global) n q v%V)
-                           (at level 20, q at level 5, format "n ↦[wg]{ q } v").
-Notation "n ↦[wg] v" := (mapsto (L:=N) (V:=global) n (DfracOwn 1) v%V)
-                      (at level 20, format "n ↦[wg] v") .
-Notation " ↪[frame]{ q } v" := (ghost_map_elem frameGName tt q v%V)
-                           (at level 20, q at level 5, format " ↪[frame]{ q } v") .
-Notation " ↪[frame] v" := (ghost_map_elem frameGName tt (DfracOwn 1) v%V)
-                            (at level 20, format " ↪[frame] v").
-Notation "n ↦[wms][ i ] l" := (mem_block_at_pos n l i)
-                                (at level 20, format "n ↦[wms][ i ] l"): bi_scope.
 
-
-
-Notation "'WP' e @ s ; E 'CTX' i ; lh {{ Φ } }" := (wp_wasm_ctx s E e%E Φ i lh)
-  (at level 20, e, Φ, lh at level 200, only parsing) : bi_scope.
-Notation "'WP' e @ E 'CTX' i ; lh {{ Φ } }" := (wp_wasm_ctx NotStuck E e%E Φ i lh)
-  (at level 20, e, Φ, lh at level 200, only parsing) : bi_scope.
-Notation "'WP' e @ E 'CTX' i ; lh ? {{ Φ } }" := (wp_wasm_ctx MaybeStuck E e%E Φ i lh)
-  (at level 20, e, Φ, lh at level 200, only parsing) : bi_scope.
-Notation "'WP' e 'CTX' i ; lh {{ Φ } }" := (wp_wasm_ctx NotStuck ⊤ e%E Φ i lh)
-  (at level 20, e, Φ, lh at level 200, only parsing) : bi_scope.
-Notation "'WP' e 'CTX' i ; lh ? {{ Φ } }" := (wp_wasm_ctx MaybeStuck ⊤ e%E Φ i lh)
-  (at level 20, e, Φ, lh at level 200, only parsing) : bi_scope.
-Notation "'WP' e @ s ; E 'CTX_EMPTY' {{ Φ } }" := (wp_wasm_ctx s E e%E Φ 0 (LH_base [] []))
-  (at level 20, e, Φ at level 200, only parsing) : bi_scope.
-
-
-Notation "'WP' e @ s ; E 'CTX' i ; lh {{ v , Q } }" := (wp_wasm_ctx s E e%E (λ v, Q) i lh)
-  (at level 20, e, Q, lh at level 200,
-   format "'[hv' 'WP'  e  '/' @  '[' s ;  '/' E  ']' 'CTX'  '/' '[' i ;  '/' lh ']'  '/' {{  '[' v ,  '/' Q  ']' } } ']'") : bi_scope.
-Notation "'WP' e @ s ; E 'CTX_EMPTY' {{ v , Q } }" := (wp_wasm_ctx s E e%E (λ v, Q) 0 (LH_base [] []))
-  (at level 20, e, Q at level 200,
-   format "'[hv' 'WP'  e  '/' @  '[' s ;  '/' E  ']' 'CTX_EMPTY'  '/' {{  '[' v ,  '/' Q  ']' } } ']'") : bi_scope.
-Notation "'WP' e @ E 'CTX' i ; lh {{ v , Q } }" := (wp_wasm_ctx NotStuck E e%E (λ v, Q) i lh)
-  (at level 20, e, Q, lh at level 200,
-   format "'[hv' 'WP'  e  '/' @ '[' E  '/' ']' 'CTX'  '/' '[' i ;  '/' lh ']'  '/' {{  '[' v ,  '/' Q  ']' } } ']'") : bi_scope.
-Notation "'WP' e @ E 'CTX' i ; lh ? {{ v , Q } }" := (wp_wasm_ctx MaybeStuck E e%E (λ v, Q) i lh)
-  (at level 20, e, Q, lh at level 200,
-   format "'[hv' 'WP'  e  '/' @  '[' E  '/' ']' 'CTX'  '/' '[' i ;  '/' lh ']'  '/' ? {{  '[' v ,  '/' Q  ']' } } ']'") : bi_scope.
-Notation "'WP' e 'CTX' i ; lh {{ v , Q } }" := (wp_wasm_ctx NotStuck ⊤ e%E (λ v, Q) i lh)
-  (at level 20, e, Q, lh at level 200,
-   format "'[hv' 'WP'  e  '/' 'CTX'  '/' '[' i ;  '/' lh ']'  '/' {{  '[' v ,  '/' Q  ']' } } ']'") : bi_scope.
-Notation "'WP' e 'CTX' i ; lh ? {{ v , Q } }" := (wp_wasm_ctx MaybeStuck ⊤ e%E (λ v, Q) i lh)
-  (at level 20, e, Q, lh at level 200,
-   format "'[hv' 'WP'  e '/' 'CTX'  '/' '[' i ;  '/' lh ']'  '/' ? {{  '[' v ,  '/' Q  ']' } } ']'") : bi_scope.
-
-
-Notation "'WP' e @ s ; E 'FRAME' n ; f {{ Φ } }" := (wp_wasm_frame s E e%E Φ n f)
-  (at level 20, only parsing) : bi_scope.
-
-Notation "'WP' e @ s ; E 'FRAME' n ; f {{ v , Q } }" := (wp_wasm_frame s E e%E (λ v, Q) n f)
-  (at level 20, e, Q, n, f at level 200,
-    format "'[hv' 'WP'  e  '/' @  '[' s ;  '/' E  ']' 'FRAME'  '/' '[' n ; f ']'  '/' {{  '[' v ,  '/' Q  ']' } } ']'") : bi_scope.
-*)
 Section code.
 
 Definition i32const (n:Z) := AI_basic (BI_const (VAL_int32 (Wasm_int.int_of_Z i32m n))).
@@ -203,35 +115,54 @@ Definition push :=
   ].
 
 
-  
+Definition stack_map :=
+  [
+    AI_basic (BI_get_local 1) ;
+    AI_basic (BI_load T_i32 None N.zero N.zero) ;
+    AI_basic (BI_set_local 3) ;
+    AI_basic (BI_get_local 1) ;
+    i32const 4 ;
+    AI_basic (BI_binop T_i32 (Binop_i BOI_add)) ;
+    AI_basic (BI_set_local 2) ;
+    AI_basic (BI_block (Tf [] [])
+                       [BI_loop (Tf [] [])
+                                [BI_get_local 2 ;
+                                 BI_get_local 3 ;
+                                 BI_relop T_i32 (Relop_i (ROI_ge SX_U)) ;
+                                 BI_br_if 1 ;
+                                 BI_get_local 2 ;
+                                 BI_get_local 2 ;
+                                 BI_get_local 2 ;
+                                 BI_load T_i32 None N.zero N.zero ;
+                                 BI_get_local 0 ;
+                                 BI_call_indirect 1 ;
+                                 BI_store T_i32 None N.zero N.zero ;
+                                 bi32const 4 ;
+                                 BI_binop T_i32 (Binop_i BOI_add) ;
+                                 BI_set_local 2 ;
+                                 BI_br 0]
+             ])
+  ].
 
 
 
 End code.
 
 
-(* Class logrel_na_invs Σ :=
-  {
-    logrel_na_invG :> na_invG Σ;
-    logrel_nais : na_inv_pool_name;
-  }.
- Close Scope byte_scope.
- Context `{!wfuncG Σ, !wtabG Σ, !wtabsizeG Σ, !wmemG Σ, !wmemsizeG Σ, !wglobG Σ, !wframeG Σ, !wtablimitG Σ, !wmemlimitG Σ, HWP: host_program_logic, !logrel_na_invs Σ}.
- Import DummyHosts. *)
  
 Section specs.
 
-(*      Context `{!wfuncG Σ, !wtabG Σ, !wtabsizeG Σ, !wmemG Σ, !wmemsizeG Σ, !wglobG Σ, !wframeG Σ, !hvisG Σ, !hmsG Σ}.  *)
-   Context `{!wfuncG Σ, !wtabG Σ, !wtabsizeG Σ, !wmemG Σ, !wmemsizeG Σ, !wglobG Σ, !wframeG Σ, !hvisG Σ, !hmsG Σ, !logrel_na_invs Σ }. 
-  (*  Context `{!wfuncG Σ, !wtabG Σ, !wtabsizeG Σ, !wmemG Σ, !wmemsizeG Σ, !wglobG Σ, (*!wstackG Σ*)!wlocsG Σ, !winstG Σ}.  *)
+
+   Context `{!wfuncG Σ, !wtabG Σ, !wtabsizeG Σ, !wmemG Σ, !wmemsizeG Σ, !wglobG Σ, !wftablimitsG Σ, !wmemlimitG Σ, !wframeG Σ, !hvisG Σ, !hmsG Σ, !logrel_na_invs Σ }. 
 
 
 
-(*Notation "m :: l ↦ v" := (load m l N.zero 4 = Some (bits v))%I (at level 50).*)
+
+
 Definition points_to_i32 n i v :=
   (∃ a b c d, n ↦[wm][ i ] a ∗ n ↦[wm][N.add i 1] b ∗
                 n ↦[wm][N.add i 2] c ∗ n ↦[wm][N.add i 3] d ∗
-                ⌜ bits v = [a ; b ; c ; d] ⌝)%I.
+                ⌜ serialise_i32 v = [a ; b ; c ; d] ⌝)%I.
 Notation "n ↦[i32][ k ] v" := (points_to_i32 n k v) (at level 50).
 
 
@@ -241,20 +172,15 @@ Lemma of_nat_to_nat_plus a b :
 Proof. lia. Qed.
 
 Lemma i32_wms n i v :
-  types_agree T_i32 v -> 
-  n ↦[i32][ i ] v ⊣⊢ n ↦[wms][ i ]bits v.
+  n ↦[i32][ i ] v ⊣⊢ n ↦[wms][ i ]serialise_i32 v.
 Proof.
-  intros Htype.
   iSplit ; iIntros "H" ; unfold mem_block_at_pos, points_to_i32.
   - iDestruct "H" as (a b c d) "(? & ? & ? & ? & ->)".
     iSimpl.
     repeat rewrite of_nat_to_nat_plus.
     rewrite N.add_0_r.
     iFrame.
-  - remember (bits v) as bs.
-    assert (length bs = length (bits v)) ; first by rewrite Heqbs.
-    erewrite length_bits in H => //.
-    simpl in H.
+  - remember (serialise_i32 v) as bs.
     repeat destruct bs => //=.
     repeat rewrite of_nat_to_nat_plus.
     rewrite N.add_0_r.
@@ -268,34 +194,18 @@ Qed.
 
 
 
-Definition isStack v l n :=
+Definition isStack v (l : seq.seq i32) n :=
   (let st_p := (v + 4 + length l * 4)%Z in
     ⌜ (two16 | v)%Z ⌝ ∗ ⌜ (length l < two14)%Z ⌝ ∗
    N.of_nat n ↦[i32][ Z.to_N v ]
-            (value_of_int st_p) ∗
+            (Wasm_int.Int32.repr st_p) ∗
             ([∗ list] i ↦ w ∈ l,
               N.of_nat n ↦[i32][ Z.to_N (st_p - 4 - 4 * i)%Z ] w) ∗
-  (*            ∀ k, ⌜ (k >= st_p)%Z ⌝ -∗ ⌜ (k < v + 16384)%Z ⌝ -∗ ∃ bk, N.of_nat n ↦[wm][ Z.to_N k ] bk *)
             ∃ bs, ⌜ (Z.of_nat (length bs) = two16 - 4 - length l * 4)%Z ⌝ ∗ N.of_nat n↦[wms][Z.to_N st_p] bs
-                                                        
-                                                         
- )%I.
-
-(*
-Definition isStack v l n :=
-  (∃ st_p, N.of_nat n ↦[i32][ Z.to_N v ]
-                    (value_of_int st_p) ∗
-                    ⌜ ((st_p - v - 4)/4)%Z =
-             length l ⌝ ∗
-                    ([∗ list] i ↦ w ∈ l,
-                      N.of_nat n ↦[i32][ Z.to_N (st_p - 4 - 4 * i)%Z ] w) ∗
-                    ∀ k, ⌜ (k >= st_p)%Z ⌝ -∗ ⌜ (k < v + 16384)%Z ⌝ -∗ ∃ bk, N.of_nat n ↦[wm][ Z.to_N k ] bk)%I. *)
+  )%I.
 
 
 
-Notation "{{{ P }}} es {{{ v , Q }}}" :=
-  (□ ∀ Φ, P -∗ (∀ v, Q -∗ Φ v) -∗ WP es @ NotStuck ; ⊤ (*CTX_EMPTY*) {{ v, Φ v }})%I (at level 50). 
-   
 Lemma separate1 {A} (a : A) l :
   a :: l = [a] ++ l.
 Proof. done. Qed.
@@ -392,22 +302,21 @@ Qed.
 
 Lemma spec_new_stack f0 n len : 
   ⊢ {{{ ⌜ f0.(f_inst).(inst_memory) !! 0 = Some n ⌝ ∗
-                                              ⌜ length (f_locs f0) >= 1 ⌝ ∗
-                                                                       ⌜ (Wasm_int.Int32.modulus - 1)%Z <>
-                                           Wasm_int.Int32.Z_mod_modulus (ssrnat.nat_of_bin (len `div` page_size)) ⌝ ∗
-                                                                        ⌜ (len + 4 < Z.to_N (two_power_nat 32))%N ⌝ ∗
-                                                                        ⌜ (page_size | len)%N ⌝ ∗
-                                                                                              
-                                                                        
-                                                                        ↪[frame] f0 ∗
-                                                                        N.of_nat n ↦[wmlength] len }}}
+        ⌜ length (f_locs f0) >= 1 ⌝ ∗
+        ⌜ (Wasm_int.Int32.modulus - 1)%Z <>
+         Wasm_int.Int32.Z_mod_modulus (ssrnat.nat_of_bin (len `div` page_size)) ⌝ ∗
+        ⌜ (len + 4 < Z.to_N (two_power_nat 32))%N ⌝ ∗
+        ⌜ (page_size | len)%N ⌝ ∗
+        ↪[frame] f0 ∗
+        N.of_nat n ↦[wmlength] len }}}
     new_stack
     {{{ v , (∃ (k : Z), ⌜ v = immV [value_of_int k] ⌝ ∗
-                                         (⌜ (k = -1)%Z ⌝ ∗
-                                            N.of_nat n↦[wmlength] len ∨
-                                            ⌜ (0 <= k)%Z /\ (k + Z.of_N page_size <= two32)%Z ⌝ ∗
-                                            isStack k [] n ∗
-                                          N.of_nat n ↦[wmlength] (len + page_size)%N) ∗ ∃ f1, ↪[frame] f1 ∗ ⌜ f_inst f1 = f_inst f0 ⌝)%I }}}.
+                                   (⌜ (k = -1)%Z ⌝ ∗
+                                      N.of_nat n↦[wmlength] len ∨
+                                      ⌜ (0 <= k)%Z /\ (k + Z.of_N page_size <= two32)%Z ⌝ ∗
+                                     isStack k [] n ∗
+                                     N.of_nat n ↦[wmlength] (len + page_size)%N) ∗
+            ∃ f1, ↪[frame] f1 ∗ ⌜ f_inst f1 = f_inst f0 ⌝)%I }}}.
 Proof.
   iIntros "!>" (Φ) "(%Hinst & %Hflocs & %Hmod & %Hlenoverflow4 & %Hlendiv & Hframe & Hlen) HΦ".
   assert (page_size | len)%N as Hlenmod => //=.
@@ -565,7 +474,7 @@ Proof.
         iFrame. }
       remember (Wasm_int.Int32.repr (ssrnat.nat_of_bin (len `div` page_size))) as c.
       iApply wp_wand_r.        
-      instantiate (1 := λ x, ((⌜ x = immV [value_of_int (N.to_nat len)] ⌝ ∗ N.of_nat n↦[i32][ len ] (value_of_int (N.to_nat len + 4))) ∗ ↪[frame] {| f_locs := set_nth (VAL_int32 c) (f_locs f0) 0
+      instantiate (1 := λ x, ((⌜ x = immV [value_of_int (N.to_nat len)] ⌝ ∗ N.of_nat n↦[i32][ len ] (Wasm_int.Int32.repr (N.to_nat len + 4))) ∗ ↪[frame] {| f_locs := set_nth (VAL_int32 c) (f_locs f0) 0
                                                                                                                                                                        (VAL_int32 (Wasm_int.Int32.imul c (Wasm_int.Int32.repr 65536))); f_inst := f_inst f0 |} )%I).
       iSplitL "Hf Hbs".
       * { iApply wp_wasm_empty_ctx.
@@ -1030,33 +939,20 @@ Proof.
         iExists _ ; iFrame.
         done.
 Qed.
-(*        iIntros (k) "%Hk1 %Hk2".
-        iExists b.
-        unfold mem_block_at_pos.
-        iDestruct (big_sepL_delete with "Hb") as "[Hb _]".
-        instantiate (1 := b).
-        instantiate (1 := N.to_nat (Z.to_N k - len - 4)%N).
-        apply repeat_lookup.
-        lia.
-        rewrite - N2Nat.inj_add.
-        rewrite N2Nat.id.
-        replace (len + 1 + 1 + 1 + 1)%N with (len + 4)%N ; last lia.
-        replace (len + 4 + (Z.to_N k - len - 4))%N with (Z.to_N k) ; last lia.
-        iFrame.
-Qed. *)
+
 
 
 Lemma spec_is_empty f0 n v s : 
   ⊢ {{{ ⌜ f0.(f_inst).(inst_memory) !! 0 = Some n ⌝ ∗
-                                              ⌜ (f_locs f0) !! 0 = Some (value_of_int v) ⌝ ∗ 
-                                              ⌜ (0 <= v <= Wasm_int.Int32.max_unsigned - 4 - length s * 4)%Z ⌝ ∗ 
-                                                                        ↪[frame] f0 ∗
-                                                                        isStack v s n }}}
+        ⌜ (f_locs f0) !! 0 = Some (value_of_int v) ⌝ ∗ 
+        ⌜ (0 <= v <= Wasm_int.Int32.max_unsigned - 4 - length s * 4)%Z ⌝ ∗ 
+        ↪[frame] f0 ∗
+        isStack v s n }}}
     is_empty
     {{{ w, ∃ k, ⌜ w = immV [value_of_int k] ⌝ ∗ isStack v s n ∗
-                                   ⌜ (k = 1 /\ s = []) \/
+                           ⌜ (k = 1 /\ s = []) \/
                   (k = 0 /\ s <> []) ⌝ ∗
-    ∃ f1, ↪[frame] f1 ∗ ⌜ f_inst f0 = f_inst f1 ⌝}}}.
+           ∃ f1, ↪[frame] f1 ∗ ⌜ f_inst f0 = f_inst f1 ⌝}}}.
 Proof.
   iIntros "!>" (Φ) "(%Hinst & %Hlocv & %Hv & Hf & Hstack) HΦ".
   unfold is_empty.
@@ -1215,16 +1111,16 @@ Proof.
 Qed.
     
     
-Lemma spec_is_full f0 n v s : 
+Lemma spec_is_full f0 n (v : Z) (s : seq.seq i32) : 
   ⊢ {{{ ⌜ f0.(f_inst).(inst_memory) !! 0 = Some n ⌝ ∗
-                                              ⌜ (f_locs f0) !! 0 = Some (value_of_int v) ⌝ ∗ 
-                                              ⌜ (0 <= v <= Wasm_int.Int32.max_unsigned - 4 - length s * 4 )%Z ⌝ ∗ 
-                                                                        ↪[frame] f0 ∗
-                                                                        isStack v s n }}}
+        ⌜ (f_locs f0) !! 0 = Some (value_of_int v) ⌝ ∗ 
+        ⌜ (0 <= v <= Wasm_int.Int32.max_unsigned - 4 - length s * 4 )%Z ⌝ ∗ 
+        ↪[frame] f0 ∗
+        isStack v s n }}}
     is_full
     {{{ w, ∃ k, ⌜ w = immV [value_of_int k] ⌝ ∗ isStack v s n ∗
                            ⌜ k = 1 \/ (length s < two14 - 1)%Z ⌝ ∗
-                                                           ∃ f1, ↪[frame] f1 ∗ ⌜ f_inst f0 = f_inst f1⌝ }}}.
+          ∃ f1, ↪[frame] f1 ∗ ⌜ f_inst f0 = f_inst f1⌝ }}}.
 Proof.
   iIntros "!>" (Φ) "(%Hinst & %Hlocv & %Hv & Hf & Hstack) HΦ".
   unfold is_full.
@@ -1339,6 +1235,13 @@ Proof.
     unfold Integers.Wordsize_32.wordsize.
     replace (two_power_nat 32) with 4294967296%Z ; last done.
     lia.
+    split ; try lia.
+    destruct Hv.
+    apply (Z.add_le_mono v (Wasm_int.Int32.max_unsigned - 4 - length s * 4) (4 + length s * 4) (4 + length s * 4)) in H0.
+    replace (Wasm_int.Int32.max_unsigned - 4 - length s * 4)%Z with (Wasm_int.Int32.max_unsigned - (4 + length s * 4))%Z in H0 ; last lia.
+    rewrite Z.sub_add in H0.
+    rewrite Z.add_assoc in H0.
+    exact H0.
     lia.
   - iIntros (w) "[-> Hf]".
     unfold of_val, fmap, list_fmap.
@@ -1347,6 +1250,8 @@ Proof.
   - iApply wp_wand_r.
     iSplitL "Hf".
     iApply (wp_select_false with "Hf") => //.
+    rewrite Hmod.
+    done.
     instantiate (1 := λ x, ⌜ x = immV [value_of_int 1] ⌝%I).
     done.
     iIntros (w) "[-> Hf]".
@@ -1365,7 +1270,8 @@ Proof.
     unfold Wasm_int.Int32.zero.
     intro Habs.
     apply Wasm_int.Int32.repr_inv in Habs => //=.
-    rewrite <- Hmod.
+    rewrite Hmod in Habs. done.
+    rewrite Hmod.
     unfold Wasm_int.Int32.modulus.
     unfold Wasm_int.Int32.wordsize.
     unfold Integers.Wordsize_32.wordsize.
@@ -1385,7 +1291,7 @@ Proof.
     iPureIntro.
 (*    unfold two14.
     replace (16384 - 1)%Z with 16383%Z ; last done. *)
-    edestruct (Z.lt_total) as [ H | [ H | H]] => //=.    
+    edestruct (Z.lt_total) as [ H | [ H | H]] => //=.     
     rewrite H in Hmod.
     (* replace (Init.Nat.of_uint (Decimal.D1 (Decimal.D6 (Decimal.D3 (Decimal.D8 (Decimal.D3 Decimal.Nil))))) * 4)%Z with 65532%Z in Hmod ; last done. *)
     replace (v + 4 + (two14 - 1) * 4 )%Z with (v + 1 * 65536)%Z in Hmod ;
@@ -1406,6 +1312,9 @@ Proof.
                 (Decimal.D1
                    (Decimal.D6 (Decimal.D3 (Decimal.D8 (Decimal.D3 Decimal.Nil))))))) in H ;
       last done. *)
+    remember (length s) as x in *.
+    rewrite - Heqx in H.
+    clear - Hlen H.
     lia.
     iExists _ ; by iFrame.
   - assert ( 0 <= v + 4 + length s * 4 )%Z ; first lia.
@@ -1417,18 +1326,19 @@ Qed.
 
 
 
-Lemma spec_pop f0 n v a s :
+Lemma spec_pop f0 n v (a : i32) s :
   ⊢ {{{ ⌜ f0.(f_inst).(inst_memory) !! 0 = Some n ⌝
-                                              ∗ ⌜ f0.(f_locs) !! 0 = Some (value_of_int v) ⌝
-                                                                          ∗ ⌜ length f0.(f_locs) >= 2 ⌝
-                                                                                                     ∗ ⌜ (0 <= v <= Wasm_int.Int32.max_unsigned - 4 - S (length s) * 4 )%Z ⌝
-                                                                                                     ∗ ⌜ types_agree T_i32 a ⌝
-                                                                                                     ∗ isStack v (a :: s) n
-                                                                                                     ∗ ↪[frame] f0 }}}
+         ∗ ⌜ f0.(f_locs) !! 0 = Some (value_of_int v) ⌝
+         ∗ ⌜ length f0.(f_locs) >= 2 ⌝
+         ∗ ⌜ (0 <= v <= Wasm_int.Int32.max_unsigned - 4 - S (length s) * 4 )%Z ⌝
+         ∗ isStack v (a :: s) n
+         ∗ ↪[frame] f0 }}}
     pop
-    {{{ w, ⌜ w = immV [a] ⌝ ∗ isStack v s n ∗ ∃ f1, ↪[frame] f1 ∗ ⌜ f_inst f0 = f_inst f1 ⌝ }}}.
+    {{{ w, ⌜ w = immV [VAL_int32 a] ⌝ ∗
+                      isStack v s n ∗
+                      ∃ f1, ↪[frame] f1 ∗ ⌜ f_inst f0 = f_inst f1 ⌝ }}}.
 Proof.
-  iIntros "!>" (Φ) "(%Hinst & %Hlocv & %Hlocs & %Hv & %Ha & Hstack & Hf) HΦ".
+  iIntros "!>" (Φ) "(%Hinst & %Hlocv & %Hlocs & %Hv & Hstack & Hf) HΦ".
   unfold pop.
   rewrite (separate1 (AI_basic _)).
   iApply wp_seq.
@@ -1441,28 +1351,30 @@ Proof.
     iSimpl.
     rewrite separate2.
     iApply wp_seq.
-    instantiate ( 1 := λ x, ((((⌜ x = immV [ value_of_int (v + 4 + length (a :: s) * 4)%Z] ⌝
-                                           ∗ [∗ list] i↦w ∈  (a :: s),
-                                 N.of_nat n ↦[i32][ Z.to_N (v + 4 + length (a :: s) * 4 - 4 - 4 * i)] w) ∗
-
-                                                                                                        (∃ bs, ⌜ (Z.of_nat (length bs) = two16 - 4 - length (a :: s) * 4)%Z ⌝ ∗ N.of_nat n ↦[wms][Z.to_N (v + 4 + length (a :: s) * 4)]bs)
-                              (*(∀ k, ⌜(k >= v + 4 + length (a :: s) * 4)%Z⌝ -∗
-                                                                                                         ⌜(k < v + 16384)%Z⌝ -∗ ∃ bk, N.of_nat n ↦[wm][Z.to_N k] bk) *))
-                                ∗  N.of_nat n↦[wms][(Wasm_int.N_of_uint i32m (Wasm_int.int_of_Z i32m v) + N.zero)%N]bits (value_of_int (v + 4 + length (a :: s) * 4)) )
-                               ∗ ↪[frame] f0)%I).
-    iSplitR ; first by iIntros "[[[[%Habs _] _] _] _]".
+    iSplitR ; last first.
     iDestruct "Hstack" as "(%Hdiv & %Hlen & Hv & Hs & Hrest)".
     iSplitR "HΦ".
-  - iApply wp_load => //.
-    iSplitL "Hs Hrest".
+  - iApply wp_load ; last first.
+    iSplitL "Hs Hrest" ; last first.
     iFrame.
-    done.
+    (* done.
     iFrame.
     rewrite N.add_0_r.
-    iSimpl.
+    iSimpl. *)
+    iDestruct (i32_wms with "Hv") as "Hv" => //=.
     rewrite Wasm_int.Int32.Z_mod_modulus_eq.
     rewrite Z.mod_small ; last by unfold Wasm_int.Int32.max_unsigned in Hv ; lia.
-    iDestruct (i32_wms with "Hv") as "Hv" => //.
+    instantiate (1 := VAL_int32 _) => /=.
+    rewrite N.add_0_r.
+    done.
+    iNext.
+   
+    by instantiate (1 := λ x, (⌜ x = immV _ ⌝ ∗ ( [∗ list] i↦w ∈ (a :: s)%SEQ, N.of_nat n
+                                      ↦[i32][ Z.to_N
+                                                (v + 4 + length (a :: s) * 4 - 4 - 4 * i)] w) ∗ ( ∃ bs : seq.seq byte, ⌜Z.of_nat (length bs) = (two16 - 4 - length (a :: s) * 4)%Z⌝ ∗
+              N.of_nat n↦[wms][Z.to_N (v + 4 + length (a :: s) * 4)]bs))%I) ; iFrame.
+    done.
+    done.
 (*    unfold mem_block_at_pos.
     unfold points_to_i32.
     remember (bits (value_of_int (v + 4 + length (a :: s) * 4))) as bs.
@@ -1480,7 +1392,7 @@ Proof.
     replace (N.of_nat (N.to_nat (Z.to_N v) + 2)) with (Z.to_N v + 2)%N ; last lia.
     replace (N.of_nat (N.to_nat (Z.to_N v) + 3)) with (Z.to_N v + 3)%N ; last lia.
     iFrame. *)
-  - iIntros (w) "[[[[->  Hs] Hrest] Hp] Hf]".
+  - iIntros (w) "[[(-> & Hs & Hrest) Hp] Hf]". 
     iAssert (isStack v (a :: s) n)%I with "[Hrest Hp Hs]" as "Hstack".
     unfold isStack.
     iFrame.
@@ -1524,7 +1436,10 @@ Proof.
     rewrite Wasm_int.Int32.unsigned_repr.
     unfold value_of_int.
     unfold Wasm_int.int_of_Z => //=.
-    replace (v + 4 + S (length s) * 4 - 4)%Z with (v + S (length s) * 4)%Z ; first done.
+    remember (length s) as x.
+    rewrite - Heqx.
+    clear Heqx Hlen s.
+    replace (v + 4 + S x * 4 - 4)%Z with (v + S x * 4)%Z ; first done.
     lia.
     unfold Wasm_int.Int32.max_unsigned.
     unfold Wasm_int.Int32.modulus.
@@ -1532,6 +1447,9 @@ Proof.
     unfold Integers.Wordsize_32.wordsize.
     replace (two_power_nat 32) with 4294967296%Z ; last done.
     lia.
+    remember (length s) as x.
+    rewrite - Heqx.
+    clear Heqx Hlen s.
     lia.
   - iIntros (w) "[-> Hf]".
     unfold of_val, fmap, list_fmap.
@@ -1554,18 +1472,43 @@ Proof.
     unfold of_val, fmap, list_fmap.
     iSimpl.
     rewrite separate2.
-    iApply (wp_seq _ _ _ (λ x, (((⌜ x = immV [a] ⌝ ∗ N.of_nat n ↦[i32][Z.to_N v] value_of_int (v + 4 + length (a :: s) * 4) ∗ ([∗ list] i↦w ∈ s, N.of_nat n ↦[i32][ Z.to_N (v + 4 + (length s) * 4 - 4 - 4 * i)] w) ∗ (∃ bs, ⌜ (Z.of_nat (length bs) = two16 - 4 - length (a :: s) * 4)%Z ⌝ ∗ N.of_nat n↦[wms][Z.to_N (v + 4 + length (a :: s) * 4)] bs) (* (∀ k, ⌜ (k >= v + 4 + length (a :: s) * 4)%Z⌝ -∗ ⌜ (k < v + 16384)%Z⌝ -∗ ∃ bk, N.of_nat n↦[wm][Z.to_N k]bk) *)) ∗
-                                                                                                                                                                                                                                                                                                                                  N.of_nat n ↦[wms][Wasm_int.N_of_uint i32m (Wasm_int.int_of_Z i32m (v + S (length s) * 4)) + N.zero] bits a )∗ ↪[frame] f1 )%I)).
+    iApply wp_seq.
     iDestruct "Hstack" as "(_ & _ & Hp & Hs & Hrest)".
-    iSplitR ; first by iIntros "[[[%Habs _] _] _]".
+    iSplitR ; last first.
     iSplitR "HΦ".
-  - iApply wp_load => //.
-    by subst f1 => //=.
+  - iApply wp_load ; last first.
     iFrame.
     rewrite separate1.
     iDestruct (big_sepL_app with "Hs") as "[Ha Hs]".
-    iSplitR "Ha".
-    iSplitR => //=.
+    iSplitR "Ha" ; last first.
+    instantiate (1 := VAL_int32 _) => /=.
+    iApply i32_wms.
+    rewrite Wasm_int.Int32.Z_mod_modulus_eq Z.mod_small.
+    rewrite N.add_0_r Z.mul_0_r Z.sub_0_r.
+    iDestruct "Ha" as "[Ha _]".
+    remember (length s) as x.
+    rewrite - Heqx.
+    clear Heqx Hlen s.
+    replace (v + 4 + S x * 4 - 4)%Z with (v + S x * 4)%Z.
+    done.
+    lia.
+    unfold Wasm_int.Int32.max_unsigned in Hv. 
+    remember (length s) as x.
+    rewrite - Heqx.
+    clear Heqx Hlen s.
+    lia.
+    by instantiate (1 := λ x, (⌜ x = immV _ ⌝ ∗ N.of_nat n
+                                          ↦[i32][ Z.to_N v] Wasm_int.Int32.repr (v + 4 + length ([a] ++ s)%list * 4) ∗
+                                          ( ∃ bs : seq.seq byte,
+                                              ⌜Z.of_nat (length bs) = (two16 - 4 - length ([a] ++ s)%list * 4)%Z⌝ ∗
+                                                                                                              N.of_nat n↦[wms][Z.to_N (v + 4 + length ([a] ++ s)%list * 4)]bs) ∗
+                                          ([∗ list] k↦y ∈ s, N.of_nat n
+                           ↦[i32][ Z.to_N
+                                     (v + 4 + length ([a] ++ s)%list * 4 - 4 -
+                                        4 * (length [a] + k)%nat)] y))%I) ; iFrame.
+    done.
+    done.
+ (*   iSplitR => //=.
     iApply (big_sepL_impl with "Hs").
     iNext. iIntros "!>" (k x) "%Hlookup Hp".
     replace (v + 4 + S (length s) * 4 - 4 - 4 * S k)%Z
@@ -1580,7 +1523,7 @@ Proof.
     rewrite Z.mul_0_r.
     rewrite Z.sub_0_r.
     replace (v + 4 + S (length s) * 4 - 4)%Z with (v + S (length s) * 4)%Z ; last lia.
-    done.
+    done. *)
 (*    replace (N.of_nat (N.to_nat (Z.to_N (v + S (length s) * 4)) + 0))
       with (Z.to_N (v + S (length s) * 4)) ; last lia.
     replace (N.of_nat (N.to_nat (Z.to_N (v + S (length s) * 4)) + 1))
@@ -1592,19 +1535,19 @@ Proof.
     iFrame.
     unfold Wasm_int.Int32.max_unsigned in Hv.
     lia. *)
-  - iIntros (w) "[[(-> & Hp & Hs & Hrest) Ha] Hf]".
+  - iIntros (w) "[[(-> & Hp & Hrest & Hs) Ha] Hf]".
     unfold of_val, fmap, list_fmap.
     iSimpl.
     rewrite separate2.
     iApply wp_seq.
-    instantiate (1 := λ x, (⌜ x = immV [a ; value_of_int v] ⌝ ∗ ↪[frame] f1)%I).
+    instantiate (1 := λ x, (⌜ x = immV [VAL_int32 a ; value_of_int v] ⌝ ∗ ↪[frame] f1)%I).
     iSplitR ; first by iIntros "[%Habs _]".
     iSplitL "Hf".
   - rewrite separate1.
     iApply wp_val_app => //.
     iSplitR ; first by iIntros "!> [%Habs _]".
+    subst.
     iApply (wp_get_local with "Hf") => //=.
-    subst f1 => //=.
     unfold set_nth.
     destruct (f_locs f0) => //=.
   - iIntros (w) "[-> Hf]".
@@ -1612,7 +1555,7 @@ Proof.
     iSimpl.
     rewrite separate3.
     iApply wp_seq.
-    instantiate (1 := λ x, (⌜ x = immV [a ; value_of_int v ;
+    instantiate (1 := λ x, (⌜ x = immV [VAL_int32 a ; value_of_int v ;
                                         value_of_int (v + S (length s) * 4)] ⌝ ∗
                                        ↪[frame] f1)%I).
     iSplitR ; first by iIntros "[%Habs _]".
@@ -1630,7 +1573,7 @@ Proof.
     iSplitL "Hp Hf".
   - rewrite (separate1 (AI_basic _)).
     iApply wp_val_app => //.
-    instantiate (1 := λ x, ((⌜ x = immV [a] ⌝ ∗
+    instantiate (1 := λ x, ((⌜ x = immV [VAL_int32 a] ⌝ ∗
                                        N.of_nat n↦[wms][Wasm_int.N_of_uint i32m
                                                                            (Wasm_int.int_of_Z i32m v) + N.zero]bits (value_of_int (v + S (length s) * 4))) ∗
                                                                                                                                                            ↪[frame] f1)%I).
@@ -1664,7 +1607,8 @@ Proof.
     simpl in Hlen.
     iSplitR "Hf".
     repeat iSplit => //.
-    iPureIntro. lia.
+    iPureIntro.
+    remember (length s) as x. rewrite - Heqx in Hlen ; clear Heqx s ; lia.
     iFrame.
     iSplitL "Hp".
   - simpl. rewrite Wasm_int.Int32.Z_mod_modulus_eq.
@@ -1672,7 +1616,8 @@ Proof.
     rewrite N.add_0_r.
     iApply i32_wms => //.
     unfold value_of_int => /=.
-    replace (v + S (length s) * 4)%Z with (v + 4 + length s * 4)%Z ; last lia.
+    remember (length s) as x. rewrite - Heqx ; clear Heqx Hlen s.
+    replace (v + S (x) * 4)%Z with (v + 4 + x * 4)%Z ; last lia.
     done.
 (*    unfold mem_block_at_pos.
     unfold points_to_i32.
@@ -1689,15 +1634,27 @@ Proof.
     iFrame.
     done. *)
   - iDestruct "Hrest" as (bs) "[%Hbs Hrest]".
-    iExists (bits a ++ bs).
+    iSplitL "Hs".
+    iApply (big_sepL_impl with "Hs").
+    iIntros "!>" (k y) "% H".
+    simpl.
+    remember (length s) as x ; rewrite - Heqx ; clear Heqx Hbs H Hlen s.
+    replace ( v + 4 + S x * 4 - 4 - 4 * S k)%Z with
+      (v + 4 + x * 4 - 4 - 4 * k)%Z.
+    done.
+    lia.
+    iExists (serialise_i32 a ++ bs).
+    iFrame.
     iSplitR.
     iPureIntro.
     rewrite app_length.
     simpl in Hbs.
     rewrite - (Nat2Z.id (length bs)).
     rewrite Hbs.
-    erewrite length_bits => //.
-    unfold t_length.
+    remember (serialise_i32 a) as l.
+    repeat (destruct l ; first done).
+    destruct l ; last done.
+    simpl.
     lia.
     unfold mem_block_at_pos.
     rewrite big_sepL_app.
@@ -1709,58 +1666,24 @@ Proof.
     rewrite of_nat_to_nat_plus.
     unfold Wasm_int.N_of_uint => //=.
     rewrite Wasm_int.Int32.Z_mod_modulus_eq.
-    rewrite Z.mod_small ; last by unfold Wasm_int.Int32.max_unsigned in Hv ; lia.
-    replace (v + S (length s) * 4)%Z with (v + 4 + length s * 4)%Z ; last lia.
+    rewrite Z.mod_small ; last by unfold Wasm_int.Int32.max_unsigned in Hv ; remember (length s) as y ; rewrite - Heqy ; clear Heqy Hbs Hlen s ; lia.
+    remember (length s) as y ; rewrite - Heqy ; clear Heqy Hbs Hlen s.
+    replace (v + S (y) * 4)%Z with (v + 4 + y * 4)%Z ; last lia.
     done.
     iApply (big_sepL_impl with "Hrest").
     iIntros "!>" (k x) "%Hbits H".
     repeat rewrite of_nat_to_nat_plus.
-    erewrite length_bits => //.
-    unfold t_length.
-    replace (Z.to_N (v + 4 + length (a :: s) * 4) + N.of_nat k)%N
-      with (Z.to_N (v + 4 + length s * 4) + N.of_nat (4+k))%N ; first done.
+    remember (serialise_i32 a) as l.
+    repeat (destruct l => //).
+    simpl.
+    remember (length s) as y ; rewrite - Heqy ; clear Heqy Hbs Hlen s.
+    replace (Z.to_N (v + 4 + S y * 4) + N.of_nat k)%N
+      with (Z.to_N (v + 4 + y * 4) + N.of_nat (4+k))%N ; first done.
     simpl.
     lia.
     iExists _ ; by subst ; iFrame.
+    all : try by iIntros "[[[% _] _] _]".
 Qed.    
-    
-
-(* 
-
-
-    iIntros (k) "%Hkm %HkM".
-    destruct (decide (k >= v + 4 + S (length s) * 4)%Z).
-    iApply "Hrest" => //=.
-    unfold mem_block_at_pos.
-    remember (bits a) as bs.
-    assert (length bs = length (bits a)) ; first by rewrite Heqbs.
-    erewrite length_bits in H => //=.
-    simpl in H.
-    repeat destruct bs => //=.
-    rewrite Wasm_int.Int32.Z_mod_modulus_eq.
-    rewrite Z.mod_small ; last by unfold Wasm_int.Int32.max_unsigned in Hv; lia.
-    rewrite N.add_0_r.
-    repeat rewrite of_nat_to_nat_plus.
-    rewrite N.add_0_r.
-    iDestruct "Ha" as "(? & ? & ? & ? & _)".
-    destruct (Z.to_nat (k - v - 4 - length s * 4)%Z) eqn:Hk.
-    assert (Z.to_N k = Z.to_N (v + S (length s) * 4)) ; first lia.
-    iExists _.
-    by rewrite H0.
-    destruct n1.
-    assert ( Z.to_N k = Z.to_N (v + S (length s) * 4) + 1)%N ; first lia.
-    iExists _.
-    by rewrite H0.
-    destruct n1.
-    assert ( Z.to_N k = Z.to_N (v + S (length s) * 4) + 2)%N ; first lia.
-    iExists _.
-    by rewrite H0.
-    destruct n1.
-    assert ( Z.to_N k = Z.to_N (v + S (length s) * 4) + 3)%N ; first lia.
-    iExists _.
-    by rewrite H0.
-    lia.
-Qed. *)
     
     
 
@@ -1768,20 +1691,21 @@ Qed. *)
                                                                          
                                                                         
     
-Lemma spec_push f0 n v a s :
+Lemma spec_push f0 n v (a : i32) s :
   ⊢ {{{ ⌜ f0.(f_inst).(inst_memory) !! 0 = Some n ⌝
-                                              ∗ ⌜ f0.(f_locs) !! 0 = Some a ⌝ 
-                                              ∗ ⌜ f0.(f_locs) !! 1 = Some (value_of_int v) ⌝
-                                                                          ∗ ⌜ length f0.(f_locs) >= 3 ⌝
-                                                                                                     ∗ ⌜ (0 <= v <= Wasm_int.Int32.max_unsigned - 4 - S (length s) * 4 )%Z ⌝
-                                                                                                     ∗ ⌜ types_agree T_i32 a ⌝
-                                                                                                     ∗ ⌜ (length s < two14 - 1)%Z ⌝
-                                                                                                     ∗ isStack v s n
-                                                                                                     ∗ ↪[frame] f0 }}}
+         ∗ ⌜ f0.(f_locs) !! 0 = Some (VAL_int32 a) ⌝ 
+         ∗ ⌜ f0.(f_locs) !! 1 = Some (value_of_int v) ⌝
+         ∗ ⌜ length f0.(f_locs) >= 3 ⌝
+         ∗ ⌜ (0 <= v <= Wasm_int.Int32.max_unsigned - 4 - S (length s) * 4 )%Z ⌝
+         ∗ ⌜ (length s < two14 - 1)%Z ⌝
+         ∗ isStack v s n
+         ∗ ↪[frame] f0 }}}
     push
-    {{{ w, ⌜ w = immV [] ⌝ ∗ isStack v (a :: s) n ∗ ∃ f1, ↪[frame] f1 ∗ ⌜ f_inst f0 = f_inst f1 ⌝ }}}. 
+    {{{ w, ⌜ w = immV [] ⌝ ∗
+           isStack v (a :: s) n ∗
+           ∃ f1, ↪[frame] f1 ∗ ⌜ f_inst f0 = f_inst f1 ⌝ }}}. 
 Proof.
-  iIntros "!>" (Φ) "(%Hinst & %Hloca & %Hlocv & %Hlocs & %Hv & %Ha & %Hlens & Hstack & Hf) HΦ".
+  iIntros "!>" (Φ) "(%Hinst & %Hloca & %Hlocv & %Hlocs & %Hv & %Hlens & Hstack & Hf) HΦ".
   unfold push.
   rewrite (separate1 (AI_basic _)).
   iApply wp_seq.
@@ -1880,14 +1804,13 @@ Proof.
     rewrite separate2.
     iApply wp_seq.
     instantiate (1 := λ x, (⌜ x = immV [value_of_int (v + 4 + length s * 4) ;
-                                        a] ⌝ ∗ ↪[frame] f1)%I).
+                                        VAL_int32 a] ⌝ ∗ ↪[frame] f1)%I).
     iSplitR ; first by iIntros "[%Habs _]".
     iSplitL "Hf".
   - rewrite separate1.
     iApply wp_val_app => //.
     iSplitR ; first by iIntros "!> [%Habs _]".
-    iApply (wp_get_local with "Hf") => //.
-    subst f1 => /=.
+    subst f1 ; iApply (wp_get_local with "Hf") => //.
     unfold set_nth.
     destruct (f_locs f0) => //=.
   - iIntros (w) "[-> Hf]".
@@ -1895,24 +1818,70 @@ Proof.
     iSimpl.
     rewrite separate3.
     iApply wp_seq.
-    instantiate
-      (1 := λ x, (((⌜ x = immV [] ⌝ ∗ N.of_nat n↦[i32][ Z.to_N v] value_of_int (v+4+length s * 4) ∗ ([∗ list] i↦w ∈ s, N.of_nat n↦[i32][Z.to_N (v + 4 + length s * 4 - 4 - 4 * i)] w) ∗ (∃ bs, ⌜ Z.of_nat (length bs) = (two16 - 4 - length (s) * 4 - 4)%Z ⌝ ∗ N.of_nat n↦[wms][Z.to_N (v + 4 + S (length s) * 4)]bs) (* (∀ k, ⌜ (k >= v + 4 + S (length s) * 4)%Z ⌝ -∗ ⌜ (k < v + 16384)%Z ⌝ -∗ ∃ bk, N.of_nat n↦[wm][Z.to_N k]bk) *))
-                     ∗ N.of_nat n ↦[wms][Wasm_int.N_of_uint i32m (Wasm_int.int_of_Z i32m (v + 4 + length s * 4)%Z) + N.zero]bits a) ∗ ↪[frame] f1)%I).
-    iSplitR ; first by iIntros "[[[ %Habs _ ] _] _]".
+   instantiate
+      (1 := λ x, (((⌜ x = immV [] ⌝ ∗ N.of_nat n↦[i32][ Z.to_N v] Wasm_int.Int32.repr (v+4+length s * 4) ∗ ([∗ list] i↦w ∈ s, N.of_nat n↦[i32][Z.to_N (v + 4 + length s * 4 - 4 - 4 * i)] w) ∗ (∃ bs, ⌜ Z.of_nat (length bs) = (two16 - 4 - length (s) * 4 - 4)%Z ⌝ ∗ N.of_nat n↦[wms][Z.to_N (v + 4 + S (length s) * 4)]bs) (* (∀ k, ⌜ (k >= v + 4 + S (length s) * 4)%Z ⌝ -∗ ⌜ (k < v + 16384)%Z ⌝ -∗ ∃ bk, N.of_nat n↦[wm][Z.to_N k]bk) *))
+                     ∗ N.of_nat n ↦[wms][Wasm_int.N_of_uint i32m (Wasm_int.int_of_Z i32m (v + 4 + length s * 4)%Z) + N.zero]bits (VAL_int32 a)) ∗ ↪[frame] f1)%I).
+    iSplitR ; first by iIntros "[[[ %Habs _ ] _] _]". 
     iDestruct "Hstack" as "(_ & _ & Hp & Hs & Hrest)".
     iDestruct "Hrest" as (bs) "[%Hbs Hrest]".
     unfold two16 in Hbs.
     unfold two14 in Hlens.
-    do 4 (destruct bs ; first by simpl in Hbs ; lia).
+    remember (length s) as x.
+    do 4 (destruct bs ; first by exfalso ; clear Heqx s ; simpl in Hbs ; lia).
     rewrite separate4.
     unfold mem_block_at_pos at 1.
     rewrite big_sepL_app.
     iDestruct "Hrest" as "[Ha Hrest]".
     iSplitR "HΦ".
-  - iApply wp_store => //.
-    instantiate (1 := [b ; b0 ; b1 ; b2]) => //=.
-    subst f1 => //=.
+  - iApply wp_wand_r. iSplitL. iApply wp_store ; last first.
     iFrame.
+    iSplitR "Ha".
+    iNext.
+    simpl.
+    subst x.
+    by instantiate (1 := λ x, (⌜ x = immV [] ⌝ ∗ N.of_nat n ↦[i32][ Z.to_N v] Wasm_int.Int32.repr (v + 4 + length s * 4) ∗ ([∗ list] i↦w ∈ s, N.of_nat n
+                           ↦[i32][ Z.to_N (v + 4 + length s * 4 - 4 - 4 * i)] w) ∗ ([∗ list] k↦y ∈ bs, N.of_nat n↦[wm][N.of_nat
+                                                 (N.to_nat
+                                                    (Z.to_N (v + 4 + length s * 4)) +
+                                                  S (S (S (S k))))]y))%I);
+    iFrame.
+    3: instantiate (1 := [b ; b0 ; b1 ; b2]) => //=. 
+    3: done.
+    2: subst f1 => //=.
+    iApply (big_sepL_impl with "Ha").
+    iIntros "!>" (k y) "% H".
+    rewrite of_nat_to_nat_plus.
+    simpl.
+    rewrite Wasm_int.Int32.Z_mod_modulus_eq Z.mod_small.
+    rewrite of_nat_to_nat_plus.
+    rewrite N.add_0_r.
+    by subst x.
+    unfold Wasm_int.Int32.max_unsigned in Hv.
+    rewrite - Heqx.
+    lia.
+    iIntros (w) "[[(-> & Hp & Hs & Hrest) Ha] Hf]".
+    iFrame.
+    iSplitR "Ha".
+    iSplit ; first done.
+    subst x ; iFrame.
+    iExists bs.
+    iSplit ; first iPureIntro.
+    simpl in Hbs.
+    remember (length s) as x.
+    rewrite - Heqx in Hbs.
+    unfold two16. lia.
+    iApply (big_sepL_impl with "Hrest").
+    iIntros "!>" (k x) "% H".
+    do 2 rewrite of_nat_to_nat_plus.
+    remember (length s) as y.
+    clear Heqy s.
+    replace (Z.to_N (v + 4 + y * 4) + N.of_nat (S (S (S (S k)))))%N with
+      (Z.to_N (v + 4 + S y * 4) + N.of_nat k)%N.
+    done.
+    lia.
+    by subst x.
+    
+(*    rewrite N2Nat.id.
     iSplitR "Ha".
     iSplit => //=.
     iExists bs.
@@ -1936,7 +1905,7 @@ Proof.
     rewrite Wasm_int.Int32.Z_mod_modulus_eq.
     rewrite Z.mod_small ; last by unfold Wasm_int.Int32.max_unsigned in Hv ; lia.
     rewrite N.add_0_r.
-    done.
+    done. *)
   - iIntros (w) "[[(-> & Hp & Hs & Hrest) Ha] Hf]".
     unfold of_val, fmap, list_fmap.
     iSimpl.
@@ -1966,6 +1935,7 @@ Proof.
     iApply (wp_get_local with "Hf") => //.
     subst f1 => //=.
     rewrite set_nth_read => //=.
+    by subst x.
   - iIntros (w) "[-> Hf]".
     unfold of_val, fmap, list_fmap.
     iSimpl.
@@ -1982,15 +1952,17 @@ Proof.
     iApply (wp_binop with "Hf") => //=.
     iPureIntro.
     unfold Wasm_int.Int32.iadd, Wasm_int.Int32.add.
-    rewrite Wasm_int.Int32.unsigned_repr ; last lia.
+    rewrite Wasm_int.Int32.unsigned_repr.
     rewrite Wasm_int.Int32.unsigned_repr.
     unfold value_of_int => //=.
-    replace (v + 4 + length s * 4 + 4)%Z with (v + 4 + S (length s) * 4)%Z => //=.
+    rewrite - Heqx.
+    replace (v + 4 + x * 4 + 4)%Z with (v + 4 + S x * 4)%Z => //=.
     lia.
     unfold Wasm_int.Int32.max_unsigned, Wasm_int.Int32.modulus.
     unfold Wasm_int.Int32.wordsize, Integers.Wordsize_32.wordsize.
     replace (two_power_nat 32) with two32 ; last done.
     unfold two32 ; lia.
+    rewrite - Heqx. lia.
   - iIntros (w) "[-> Hf]".
     unfold of_val, fmap, list_fmap.
     iSimpl.
@@ -2008,14 +1980,14 @@ Proof.
     rewrite Z.mod_small ; last by unfold Wasm_int.Int32.max_unsigned in Hv ; lia.
     iDestruct (i32_wms with "Hp") as "Hp" => //.
     rewrite N.add_0_r.
-    unfold value_of_int => //=.
+    by subst x.
   - iIntros (w) "[[-> Hp] Hf]".
     iApply "HΦ".
     iSplit => //=.
     unfold isStack.
     iSplitR "Hf".
     repeat iSplit => //=.
-    iPureIntro ; unfold two14 ; lia.
+    iPureIntro ; rewrite - Heqx ; clear Heqx s ; unfold two14 ; lia.
     iSplitL "Hp".
     rewrite Wasm_int.Int32.Z_mod_modulus_eq.
     rewrite Z.mod_small ; last by unfold Wasm_int.Int32.max_unsigned in Hv ; lia.
@@ -2028,21 +2000,959 @@ Proof.
     rewrite Wasm_int.Int32.Z_mod_modulus_eq.
     rewrite Z.mod_small ; last by unfold Wasm_int.Int32.max_unsigned in Hv ; lia.
     rewrite N.add_0_r.
-    replace (v + 4 + S (length s) * 4 - 4 - 4 * 0%nat)%Z
-      with (v + 4 + length s * 4)%Z ; last lia.
+    rewrite - Heqx.
+    replace (v + 4 + S x * 4 - 4 - 4 * 0%nat)%Z
+      with (v + 4 + x * 4)%Z ; last lia.
     done.
     iApply (big_sepL_impl with "Hs").
-    iIntros "!>" (k x) "%Hbits H".
-    replace (v + 4 + S (length s) * 4 - 4 - 4 * S k)%Z
-      with  (v + 4 + length s * 4 - 4 - 4 * k)%Z ; last lia.
+    iIntros "!>" (k y) "%Hbits H".
+    rewrite - Heqx.
+    replace (v + 4 + S x * 4 - 4 - 4 * S k)%Z
+      with  (v + 4 + x * 4 - 4 - 4 * k)%Z ; last lia.
     done.
     iDestruct "Hrest" as (bs0) "[%Hbs0 Hrest]".
     iExists bs0.
     iSplit => //=.
     iPureIntro.
+    rewrite - Heqx.
     lia.
+    by subst x.
     iExists _ ; by subst ; iFrame.
 Qed.
+
+
+Fixpoint stackAll {A} (s : seq.seq A) (Φ : A -> iPropI Σ) : iPropI Σ :=
+  match s with
+  | [] => (True)%I
+  | a :: s => (Φ a ∗ stackAll s Φ)%I
+  end.
+
+
+Fixpoint stackAll2 {A} s1 s2 (Ψ : A -> A -> iPropI Σ) :=
+  match s1, s2 with
+  | [], [] => True%I
+  | a1 :: s1, a2 :: s2 => (Ψ a1 a2 ∗ stackAll2 s1 s2 Ψ)%I
+  | _, _ => False%I
+  end.
+
+
+Lemma stackAll_app {A} (s : seq.seq A) s' Φ :
+  ⊢ stackAll (s ++ s') Φ ∗-∗ stackAll s Φ ∗ stackAll s' Φ.
+Proof.
+  iSplit.
+  - iIntros "H".
+    induction s => //=.
+    by iFrame.
+    iDestruct "H" as "[? H]".
+    iFrame.
+    exact IHs.
+  - iIntros "[Hs Hs']".
+    induction s => //=.
+    iDestruct "Hs" as "[? Hs]".
+    iFrame.
+    exact IHs.
+Qed.
+
+    
+
+
+Lemma drop_is_nil {A} n (s : seq.seq A) :
+  drop n s = [] -> n >= length s.
+Proof.
+  generalize dependent n.
+  induction s ; intros => //=.
+  lia.
+  destruct n => //=.
+  simpl in H.
+  apply IHs in H.
+  lia.
+Qed.
+
+Lemma in_take {A} n s (x : A) :
+  In x (take n s) -> In x s.
+Proof.
+  generalize dependent s.
+  induction n ; intro s => //=.
+  destruct s => //=.
+  intros [H | H] ; first (by left) ; apply IHn in H ; by right.
+Qed.
+  
+  
+
+
+Lemma spec_stack_map (f0 : frame) (n : immediate) (f : i32) (v : Z) (s : seq.seq i32)
+      j0 a cl 
+      (Φ : i32 -> iPropI Σ) (Ψ : i32 -> i32 -> iPropI Σ) :
+  ⊢ {{{  ⌜ f0.(f_inst).(inst_memory) !! 0 = Some n ⌝  ∗
+            ⌜ f0.(f_locs) !! 0 = Some (VAL_int32 f) ⌝  ∗
+            ⌜ f0.(f_locs) !! 1 = Some (value_of_int v) ⌝ ∗
+            ⌜ length f0.(f_locs) >= 4 ⌝ ∗
+            ⌜ (0 <= v)%Z ⌝ ∗                                   
+            ⌜ (v + 4 + length s * 4 ≤ Wasm_int.Int32.max_unsigned)%Z ⌝ ∗
+            isStack v s n ∗
+            stackAll s Φ ∗
+            ⌜ f0.(f_inst).(inst_types) !! 1 = Some (Tf [T_i32] [T_i32]) ⌝ ∗
+
+            ⌜ f0.(f_inst).(inst_tab) !! 0 = Some j0 ⌝ ∗
+            (N.of_nat j0) ↦[wt][ N.of_nat (Wasm_int.nat_of_uint i32m f) ] (Some a) ∗
+            (N.of_nat a) ↦[wf] cl ∗
+            ⌜ match cl with FC_func_native _ t _ _ => t | FC_func_host t _ => t end
+         = Tf [T_i32] [T_i32] ⌝ ∗ 
+            (∀ (u : i32) (fc : frame),
+                {{{ Φ u ∗
+                      ⌜ f_inst f0 = f_inst fc ⌝ ∗
+                       ↪[frame] fc ∗
+                       (N.of_nat j0) ↦[wt][ N.of_nat (Wasm_int.nat_of_uint i32m f) ] (Some a) ∗
+                       (N.of_nat a) ↦[wf] cl
+                  }}}
+                  [ AI_basic (BI_const (VAL_int32 u)) ;
+                    AI_invoke a ]
+                  {{{ w, (∃ v, ⌜ w = immV [VAL_int32 v] ⌝ ∗ Ψ u v)
+                           ∗ ↪[frame] fc
+                           ∗ (N.of_nat j0) ↦[wt][ N.of_nat (Wasm_int.nat_of_uint i32m f) ] (Some a) 
+                           ∗ (N.of_nat a) ↦[wf] cl }}}) ∗   
+            ↪[frame] f0 }}}
+    stack_map
+    {{{ w, ⌜ w = immV [] ⌝ ∗
+           (∃ s', isStack v s' n ∗ stackAll2 s s' Ψ) ∗
+           (∃ f1, ↪[frame] f1 ∗ ⌜ f_inst f0 = f_inst f1 ⌝ )
+    }}}.
+Proof.
+  iIntros "!>" (Ξ) "(%Hinstmem & %Hlocs0 & %Hlocs1 & %Hlocs & %Hvb & %Hv & Hs & HΦ & %Htypes & %Htab & Htab & Hcl & %Hclt & #Hspec & Hf) HΞ".
+  unfold stack_map.
+  rewrite (separate1 (AI_basic (BI_get_local 1))).
+  iApply wp_seq.
+  iSplitR ; last first.
+  iSplitL "Hf".
+  iApply wp_get_local => //.
+  instantiate (1 := λ x, x = immV [value_of_int v]) => //.
+  iIntros (w) "[-> Hf]".
+  iSimpl.
+  rewrite (separate2 (i32const v)).
+  iApply wp_seq.
+  iSplitR ; last first.
+  iSplitL "Hf Hs".
+  iApply wp_load => // ; last first.
+  unfold isStack.
+  iDestruct "Hs" as "(% & % & Hn & ?)".
+  iDestruct (i32_wms with "Hn") as "Hn".
+  rewrite N.add_0_r.
+  simpl.
+  rewrite Wasm_int.Int32.Z_mod_modulus_eq.
+  rewrite Z.mod_small.
+  unfold bits.
+  instantiate (1 := VAL_int32 _) => /=.
+(*  unfold Wasm_int.N_of_uint, Wasm_int.int_of_Z.
+  destruct i32m.  
+  replace (N_of_uint (int_of_Z v)) with (Z.to_N v). *)
+  iFrame.
+  iNext.
+  instantiate ( 1 := λ x, (⌜ x = immV [value_of_int (v + 4 + length s * 4)] ⌝ ∗
+                                     ⌜(two16 | v)%Z⌝ ∗
+                                     ⌜(length s < two14)%Z⌝ ∗
+                                     ([∗ list] i↦w ∈ s, N.of_nat n ↦[i32][ Z.to_N (v + 4 + length s * 4 - 4 - 4 * i)] w) ∗
+      (∃ bs : seq.seq byte, ⌜Z.of_nat (length bs) = (two16 - 4 - length s * 4)%Z⌝ ∗
+                                                                              N.of_nat n↦[wms][Z.to_N (v + 4 + length s * 4)]bs))%I).
+  iFrame.
+  done.
+  unfold Wasm_int.Int32.max_unsigned in Hv ; lia.
+  done.
+  iIntros (w) "[[[-> Hs] Hn] Hf]".
+  iSimpl.
+  rewrite (separate2 (i32const (v + _ + _))).
+  iApply wp_seq.
+  iSplitR ; last first.
+  iSplitL "Hf".
+  iApply wp_set_local => //.
+  by instantiate (1 := λ x, x = immV []).
+  iIntros (w) "[-> Hf]".
+  iSimpl.
+  rewrite (separate1 (AI_basic (BI_get_local 1))).
+  iApply wp_seq.
+  iSplitR ; last first.
+  iSplitL "Hf".
+  iApply (wp_get_local with "Hf") => //=.
+  unfold set_nth.
+  destruct (f_locs f0) ; first by inversion Hlocs0.
+  destruct l ; first by inversion Hlocs1.
+  simpl in Hlocs1.
+  inversion Hlocs1 ; subst.
+  done.
+  by instantiate (1 := λ x, x = immV [value_of_int v]).
+  iIntros (w) "[-> Hf]".
+  iSimpl.
+  rewrite separate3.
+  iApply wp_seq.
+  iSplitR ; last first.
+  iSplitL "Hf".
+  iApply (wp_binop with "Hf") => //.
+  by instantiate (1 := λ x, ⌜ x = immV [_] ⌝%I).
+  iIntros (w) "[-> Hf]".
+  iSimpl.
+  rewrite (separate2 _ (AI_basic (BI_set_local 2))).
+  iApply wp_seq.
+  iSplitR ; last first.
+  iSplitL "Hf".
+  iApply wp_set_local => //=.
+  simpl.
+  rewrite length_is_size size_set_nth.
+  rewrite length_is_size in Hlocs.
+  unfold ssrnat.maxn.
+  destruct (ssrnat.leq _ _) ; lia.
+  by instantiate (1 := λ x, x = immV []).
+  iIntros (w) "[-> Hf]".
+  iSimpl.
+  rewrite - (app_nil_l [AI_basic (BI_block _ _)]).
+  iApply (wp_block with "Hf") => //.
+  iIntros "!> Hf".
+  iSimpl.
+  iApply wp_wasm_empty_ctx.
+  rewrite - (cat0s [AI_basic (BI_loop _ _)]) - (cats0 [AI_basic (BI_loop _ _)]).
+  iApply wp_label_push ; first done.
+  (*rewrite - (cats0 [AI_basic (BI_loop _ _)]).
+  iApply wp_seq_ctx.
+  iSplitR ; last first.
+  iApply (wp_label_bind with "[Hf Hs Hn]") ; last first. 
+  iPureIntro.
+  unfold lfilled, lfill.
+  instantiate (4 := []) => /=.
+  by rewrite app_nil_r. *)
+  rewrite - (app_nil_l [AI_basic (BI_loop _ _)]).
+  iApply (wp_loop_ctx with "Hf") => //.
+  iIntros "!> Hf".
+  simpl.
+  rewrite - (cat0s (AI_basic (BI_get_local 2) :: _)).
+  rewrite - (cats0 [AI_basic _;_;_;_;_;_;_;_;_;_;_;_;_;_;_]). 
+  iApply wp_label_push ; first done.
+(*  iApply (wp_label_bind with "[Hf Hs Hn]") ; last first.
+  iPureIntro.
+  unfold lfilled, lfill.
+  instantiate (4 := []) => /=.
+  by rewrite app_nil_r.  *)
+  unfold Wasm_int.Int32.iadd, Wasm_int.Int32.add.
+  rewrite Wasm_int.Int32.unsigned_repr ; last lia.
+  rewrite Wasm_int.Int32.unsigned_repr ; last by unfold Wasm_int.Int32.max_unsigned,
+      Wasm_int.Int32.modulus, Wasm_int.Int32.wordsize, Integers.Wordsize_32.wordsize.
+  iAssert (∀ (j :nat) s', ⌜ j <= length s ⌝ -∗ ⌜ length s' = length s - j ⌝ -∗ ↪[frame] {|
+                    f_locs :=
+                      set_nth (VAL_int32 (Wasm_int.Int32.repr (v + 4 )))
+                        (set_nth
+                           (VAL_int32 (Wasm_int.Int32.repr (v + 4 + length s * 4)))
+                           (f_locs f0) 3
+                           (VAL_int32 (Wasm_int.Int32.repr (v + 4 + length s * 4)))) 2
+                        (VAL_int32 (Wasm_int.Int32.repr (v + 4 + (length s - j%Z) * 4)));
+                    f_inst := f_inst f0
+                    |} -∗
+                    isStack v (take j s ++ s') n -∗ (*  ++ drop (length s - j) s) n -∗ *)
+                    stackAll (take j s) Φ -∗
+                    stackAll2 (drop j s) s' Ψ -∗
+                    N.of_nat j0 ↦[wt][N.of_nat (Z.to_nat (Wasm_int.Int32.unsigned f))]Some a -∗
+                    N.of_nat a↦[wf] cl -∗
+                    (∀ w : val,
+                        ⌜w = immV []⌝ ∗ (∃ s' : seq.seq i32, isStack v s' n ∗ stackAll2 s s' Ψ) ∗
+                                  (∃ f1 : frame,  ↪[frame]f1 ∗ ⌜f_inst f0 = f_inst f1⌝) -∗ 
+                                  Ξ w) -∗
+                    WP [AI_basic (BI_get_local 2); AI_basic (BI_get_local 3);
+     AI_basic (BI_relop T_i32 (Relop_i (ROI_ge SX_U))); AI_basic (BI_br_if 1);
+     AI_basic (BI_get_local 2); AI_basic (BI_get_local 2); AI_basic (BI_get_local 2);
+     AI_basic (BI_load T_i32 None N.zero N.zero); AI_basic (BI_get_local 0);
+     AI_basic (BI_call_indirect 1); AI_basic (BI_store T_i32 None N.zero N.zero);
+     AI_basic (bi32const 4); AI_basic (BI_binop T_i32 (Binop_i BOI_add));
+     AI_basic (BI_set_local 2); AI_basic (BI_br 0)]
+  CTX
+  2;
+  push_base (LH_rec [] 0 [] (LH_base [] []) []) 0
+    [AI_basic
+       (BI_loop (Tf [] [])
+          [BI_get_local 2; BI_get_local 3; BI_relop T_i32 (Relop_i (ROI_ge SX_U));
+          BI_br_if 1; BI_get_local 2; BI_get_local 2; BI_get_local 2;
+          BI_load T_i32 None N.zero N.zero; BI_get_local 0; 
+          BI_call_indirect 1; BI_store T_i32 None N.zero N.zero; 
+          bi32const 4; BI_binop T_i32 (Binop_i BOI_add); BI_set_local 2; 
+          BI_br 0])] [] []
+    {{ v0, Ξ v0 }})%I as "H".
+  { iIntros (j).
+  iInduction j as [|j] "IHj".
+  { iIntros (s') "%Hj %Hs' Hf Hs HΦ HΨ Htab Hcl HΞ".
+    rewrite (separate1 (AI_basic (BI_get_local 2))).
+    iApply wp_seq_ctx.
+    iSplitR ; last first.
+    iSplitL "Hf".
+    iApply (wp_get_local with "Hf").
+    simpl. by rewrite set_nth_read.
+    by instantiate ( 1 := λ x, x = immV _).
+    iIntros (w) "[-> Hf]".
+    iSimpl.
+    rewrite (separate2 _ (AI_basic (BI_get_local 3))).
+    iApply wp_seq_ctx.
+    iSplitR ; last first.
+    iSplitL "Hf".
+    rewrite (separate1 _ [AI_basic (BI_get_local 3)]).
+    iApply wp_val_app => //.
+    iSplitR ; last first.
+    iApply wp_wand_r.
+    iSplitL.
+    iApply (wp_get_local with "Hf").
+    simpl.
+    destruct (f_locs f0) ; first by inversion Hlocs.
+    destruct l ; first by inversion Hlocs1.
+    destruct l ; first by simpl in Hlocs ; lia.
+    simpl.
+    by rewrite set_nth_read.
+    by instantiate (1 := λ x, x = immV _).
+    iIntros (w) "[-> Hf]".
+    rewrite Z.sub_0_r.
+    iSimpl.
+    instantiate (1 := λ x, (⌜ x = immV _ ⌝ ∗ ↪[frame] _)%I).
+    iFrame.
+    done.
+    by iIntros "!> [% _]".
+    iIntros (w) "[-> Hf]".
+    iSimpl.
+(*  
+  iInduction s as [|a s] "IHs".
+  { *)
+    rewrite (separate3 _ _ (AI_basic (BI_relop _ _))).
+    iApply wp_seq_ctx.
+    iSplitR ; last first.
+    iSplitL "Hf".
+    iApply (wp_relop with "Hf").
+(*    rewrite Z.mul_0_l.
+    rewrite Z.add_0_r.
+    unfold Wasm_int.Int32.iadd, Wasm_int.Int32.add.
+    rewrite Wasm_int.Int32.unsigned_repr.
+    rewrite Wasm_int.Int32.unsigned_repr. *)
+    simpl.
+    unfold Wasm_int.Int32.ltu.
+    rewrite Wasm_int.Int32.unsigned_repr.
+    rewrite Coqlib.zlt_false.
+    simpl.
+    done.
+    lia.
+    split ; try lia.
+    exact Hv.
+    (*    unfold Wasm_int.Int32.max_unsigned.
+    unfold Wasm_int.Int32.modulus.
+    unfold Wasm_int.Int32.wordsize.
+    unfold Integers.Wordsize_32.wordsize.
+    done.
+    lia. *)
+    by instantiate (1 := λ x, ⌜ x = immV _ ⌝%I).
+    iIntros (w) "[-> Hf]".
+    iSimpl.
+    rewrite - (app_nil_l (i32const _ :: _)).
+    rewrite (separate2 _ (AI_basic (BI_br_if 1))).
+    iApply wp_base_push ; first done.
+(*    iApply wp_seq_ctx.
+    iSplitR ; last first.
+    iSplitL "Hf". *)
+    iApply (wp_br_if_true_ctx with "Hf").
+    done.
+    iIntros "!> Hf".
+(*    iApply wp_value.
+    unfold IntoVal.
+    by apply of_to_val.
+    by instantiate (1 := λ x, (⌜ x = brV _ ⌝ ∗ ↪[frame] _)%I) ; iFrame.
+    iIntros (w) "[-> Hf]".
+    iSimpl. *)
+    rewrite - (app_nil_l [AI_basic (BI_br 1)]).
+    iApply (wp_br_ctx with "Hf") => //.
+    iIntros "!> Hf".
+    iApply wp_value.
+    unfold IntoVal.
+    by apply of_to_val.
+    iApply "HΞ".
+    iSplit ; first done.
+    iSplitR "Hf".
+    iExists s'.
+    unfold take.
+    unfold drop.
+    iFrame.
+    iExists _.
+(*    iSplitL ; last done.
+    unfold isStack.
+    iDestruct "Hs" as "(% & % & Hl & Hbs)".
+    iSplitR ; first done.
+    iSplitR ; first done.
+    iSplitL "Hn".
+    iApply i32_wms => //.
+    rewrite N.add_0_r.
+    rewrite Wasm_int.Int32.Z_mod_modulus_eq.
+    rewrite Z.mod_small.
+    iExact "Hn".
+    unfold Wasm_int.Int32.max_unsigned in Hv.
+    lia.
+    iFrame. 
+    iExists _. *)
+    iFrame.
+    done.
+    all : try by iIntros "[% _]". }
+  iIntros (s') "%Hj %Hs' Hf Hs HΦ HΨ Htab Hcl HΞ".
+  destruct s as [|v0 s]; first by inversion Hj.
+  cut (exists ys y, v0 :: take j s = ys ++ [y]) ;
+  [ intro Htail ; destruct Htail as (ys & y & Htail) |
+    exists (removelast (v0 :: take j s)) ;
+    exists (List.last (v0 :: take j s) (Wasm_int.Int32.repr 1)) ;
+    apply app_removelast_last ;
+    apply not_eq_sym ; apply nil_cons ].
+  simpl in Hv.
+  simpl in Hj.
+  assert (j `min` length s = j) as Hjmin.
+  { remember (length s) as x. rewrite - Heqx in Hj.
+    lia. } 
+  rewrite (separate1 (AI_basic (BI_get_local 2))).
+  iApply wp_seq_ctx.
+  iSplitR ; last first.
+  iSplitL "Hf".
+  iApply (wp_get_local with "Hf").
+  simpl. by rewrite set_nth_read.
+  by instantiate ( 1 := λ x, x = immV _).
+  iIntros (w) "[-> Hf]".
+  iSimpl.
+  rewrite (separate2 _ (AI_basic (BI_get_local 3))).
+  iApply wp_seq_ctx.
+  iSplitR ; last first.
+  iSplitL "Hf".
+  rewrite (separate1 _ [AI_basic (BI_get_local 3)]).
+  iApply wp_val_app => //.
+  iSplitR ; last first.
+  iApply wp_wand_r.
+  iSplitL.
+  iApply (wp_get_local with "Hf").
+  simpl.
+  destruct (f_locs f0) ; first by inversion Hlocs.
+  destruct l ; first by inversion Hlocs1.
+  destruct l ; first by simpl in Hlocs ; lia.
+  simpl.
+  by rewrite set_nth_read.
+  by instantiate (1 := λ x, x = immV _).
+  iIntros (w) "[-> Hf]".
+  iSimpl.
+  instantiate (1 := λ x, (⌜ x = immV _ ⌝ ∗ ↪[frame] _)%I).
+  iFrame.
+  done.
+  by iIntros "!> [% _]".
+  iIntros (w) "[-> Hf]".
+  iSimpl.
+  rewrite (separate3 _ _ (AI_basic (BI_relop _ _))).
+  iApply wp_seq_ctx.
+  iSplitR ; last first.
+  iSplitL "Hf".
+  iApply (wp_relop with "Hf").
+  simpl.
+  unfold Wasm_int.Int32.ltu.
+  rewrite Wasm_int.Int32.unsigned_repr.
+  rewrite Wasm_int.Int32.unsigned_repr.
+  rewrite Coqlib.zlt_true.
+  simpl.
+  done.
+  lia.
+  lia.
+  lia.
+  by instantiate (1 := λ x, ⌜ x = immV _ ⌝%I).
+  iIntros (w) "[-> Hf]".
+  iSimpl.
+  rewrite (separate2 (AI_basic (BI_const (VAL_int32 _)))).
+  iApply wp_seq_ctx.
+  iSplitR ; last first.
+  iSplitL "Hf".
+  iApply (wp_br_if_false with "Hf").
+  done.
+  iNext.
+  by instantiate (1 := λ x, ⌜ x = immV [] ⌝%I).
+  iIntros (w) "[-> Hf]".
+  iSimpl.
+  rewrite (separate1 (AI_basic (BI_get_local 2)) [_;_;_;_;_;_;_;_;_;_]).
+  iApply wp_seq_ctx.
+  iSplitR ; last first.
+  iSplitL "Hf".
+  iApply (wp_get_local with "Hf") => /=.
+  by rewrite set_nth_read.
+  by instantiate (1 := λ x, x = immV _).
+  iIntros (w) "[-> Hf]".
+  iSimpl.
+  rewrite (separate2 (i32const (v + 4 + _ * 4))).
+  iApply wp_seq_ctx.
+  iSplitR ; last first.
+  iSplitL "Hf".
+  rewrite (separate1 (i32const (v + 4 + _ * 4))).
+  iApply wp_val_app. done.
+  iSplitR ; last first.
+  iApply wp_wand_r.
+  iSplitL.
+  iApply (wp_get_local with "Hf") => /=.
+  by rewrite set_nth_read.
+  by instantiate (1 := λ x, x = immV _).
+  iIntros (w) "[-> Hf]".
+  iSimpl.
+  by instantiate (1 := λ x, (⌜ x = immV _ ⌝ ∗ ↪[frame] _)%I) ; iFrame.
+  by iIntros "!> [% _]".
+  iIntros (w) "[-> Hf]".
+  iSimpl.
+  rewrite (separate3 (i32const (v + 4 + _ * 4))).
+  iApply wp_seq_ctx.
+  iSplitR ; last first.
+  iSplitL "Hf".
+  rewrite (separate2 (i32const (v + 4 + _ * 4))).
+  iApply wp_val_app ; first done.
+  iSplitR ; last first.
+  iApply wp_wand_r.
+  iSplitL.
+  iApply (wp_get_local with "Hf") => /=.
+  by rewrite set_nth_read.
+  by instantiate (1 := λ x, x = immV _).
+  iIntros (w) "[-> Hf]".
+  iSimpl.
+  by instantiate (1 := λ x, (⌜ x = immV _ ⌝ ∗ ↪[frame] _)%I) ; iFrame.
+  by iIntros "!> [% _]".
+  iIntros (w) "[-> Hf]".
+  iSimpl.
+  rewrite (separate4 (i32const (v + 4 + _ * 4))).
+  iApply wp_seq_ctx.
+  iSplitR ; last first.
+  iSplitL "Hf Hs".
+  rewrite (separate2 (i32const (v + 4 + _ * 4))).
+  iApply wp_val_app ; first done.
+  iSplitR ; last first.
+ 
+  iApply wp_wand_r.
+  iSplitL.
+
+  iApply wp_load ; last first.
+  iFrame.
+  unfold isStack.
+  iDestruct "Hs" as "(Hdiv & Hlen & Hn & Hl & Hbs)".
+  rewrite cat_app.
+  iDestruct (big_sepL_app with "Hl") as "[Hs Hs']".
+  rewrite app_length.
+  rewrite Hs'.
+  rewrite take_length.
+  replace (S j `min` length (v0 :: s)) with (S j) ; last by simpl ; lia.
+  unfold take ; fold (take (A := value)).
+  rewrite Htail.
+  iDestruct (big_sepL_app with "Hs") as "[Hs H]".
+  iDestruct "H" as "[H _]".
+  iDestruct (i32_wms with "H") as "H" => //.
+  rewrite Nat.add_0_r.
+  rewrite N.add_0_r.
+  replace (Wasm_int.N_of_uint i32m (Wasm_int.Int32.repr (v + 4 + (S (length s) - S j) * 4)))
+    with (Z.to_N (v + 4 + (S (length s) - S j) * 4)).
+  replace (S j + (length (v0 :: s) - S j)) with (length (v0 :: s)) ; last by simpl ; lia.
+  replace (v + 4 + length (v0 :: s) * 4 - 4 - 4 * length ys)%Z
+    with (v + 4 + length (v0 :: s) * 4 - S (length ys) * 4)%Z ; last lia.
+  replace (S (length ys)) with (length (ys ++ [y])) ;
+    last by rewrite app_length ; simpl ; lia.
+  rewrite (cat_app ys [y]).
+  rewrite - Htail.
+  simpl.
+  rewrite firstn_length.
+  rewrite Hjmin.
+  rewrite (Z.mul_sub_distr_r (S (length s)) (S j) 4).
+  simpl in Hj.
+  remember (length s) as x.
+  rewrite - Heqx.
+  replace (v + 4 + S x * 4 - S j * 4)%Z
+    with (v + 4 + (S x * 4 - S j * 4))%Z ;
+    last lia.
+  rewrite Wasm_int.Int32.Z_mod_modulus_eq Z.mod_small.
+  instantiate (1 := VAL_int32 _).
+  iSplitR "H" ; last iExact "H".
+  iNext.
+  subst x.
+  instantiate ( 1 := λ x, (⌜ x = immV [VAL_int32 y] ⌝ ∗ ⌜ (two16 | v)%Z ⌝ ∗ ⌜ (S (length s) < two14)%Z ⌝ ∗ N.of_nat n ↦[i32][ Z.to_N v] Wasm_int.Int32.repr (v + 4 + S (length s) * 4) ∗  (∃ bs : seq.seq byte, ⌜ Z.of_nat (length bs) = (two16 - 4 - S (length s) * 4)%Z⌝ ∗
+            N.of_nat n↦[wms][Z.to_N (v + 4 + S (length s) * 4)]bs) ∗ ([∗ list] k↦y0 ∈ s', N.of_nat n
+                              ↦[i32][ Z.to_N
+                                        (v + 4 + S (length s) * 4 - 4 - 4 * S (j + k))] y0) ∗ [∗ list] k↦y0 ∈ ys, N.of_nat n
+                             ↦[i32][ Z.to_N (v + 4 + S (length s) * 4 - 4 - 4 * k)] y0)%I).
+  iFrame.
+  done.
+  simpl.
+  unfold Wasm_int.Int32.max_unsigned in Hv ; rewrite - Heqx in Hv ; lia.
+  simpl.
+  rewrite Wasm_int.Int32.Z_mod_modulus_eq.
+  rewrite Z.mod_small.
+  done.
+  unfold Wasm_int.Int32.max_unsigned in Hv ; lia.
+  done.
+  done.
+  iIntros (w) "[[[-> H1] H2] Hf]".
+  iSimpl.
+  instantiate (1 := λ x, (⌜ x = immV _ ⌝ ∗
+                                     ( ⌜(two16 | v)%Z⌝ ∗ ⌜(S (length s) < two14)%Z⌝ ∗ N.of_nat n ↦[i32][ Z.to_N v] Wasm_int.Int32.repr (v + 4 + S (length s) * 4) ∗
+         (∃ bs : seq.seq byte, ⌜Z.of_nat (length bs) = (two16 - 4 - S (length s) * 4)%Z⌝ ∗
+            N.of_nat n↦[wms][Z.to_N (v + 4 + S (length s) * 4)]bs) ∗
+         ([∗ list] k↦y0 ∈ s', N.of_nat n
+                              ↦[i32][ Z.to_N
+                                        (v + 4 + S (length s) * 4 - 4 - 4 * S (j + k))] y0) ∗
+         ([∗ list] k↦y0 ∈ ys, N.of_nat n
+                                       ↦[i32][ Z.to_N (v + 4 + S (length s) * 4 - 4 - 4 * k)] y0))
+                                     ∗ N.of_nat n↦[wms][Wasm_int.N_of_uint i32m
+                            (Wasm_int.Int32.repr (v + 4 + (length (v0 :: s) - S j) * 4)) +
+                                                          N.zero]bits (VAL_int32 y)
+                                     ∗ ↪[frame] {|
+                    f_locs :=
+                      set_nth
+                        (VAL_int32
+                           (Wasm_int.Int32.repr (v + 4)))
+                        (set_nth
+                           (VAL_int32
+                              (Wasm_int.Int32.repr (v + 4 + length (v0 :: s) * 4)))
+                           (f_locs f0) 3
+                           (VAL_int32
+                              (Wasm_int.Int32.repr (v + 4 + length (v0 :: s) * 4)))) 2
+                        (VAL_int32
+                           (Wasm_int.Int32.repr (v + 4 + (length (v0 :: s) - S j) * 4)));
+                    f_inst := f_inst f0
+                                     |})%I).
+  iFrame.
+  done.
+  by iIntros "!> [% _]".
+  iIntros (w) "(-> & (Hdiv & Hlen & Hv & Hbs & Hs' & Hs) & H & Hf)".
+  iSimpl.
+  rewrite (separate4 (i32const (v + 4 + _ * 4))).
+  iApply wp_seq_ctx.
+  iSplitR ; last first.
+  iSplitL "Hf".
+  rewrite (separate3 (i32const (v + 4 + _ * 4))).
+  iApply wp_val_app ; first done.
+  iSplitR ; last first.
+  iApply wp_wand_r.
+  iSplitL.
+  iApply (wp_get_local with "Hf") => /=.
+  destruct (f_locs f0) ; inversion Hlocs0.
+  simpl. done.
+  by instantiate (1 := λ x, x = immV _).
+  iIntros (w) "[-> Hf]".
+  iSimpl.
+  by instantiate (1 := λ x, (⌜ x = immV _ ⌝ ∗ ↪[frame] _)%I) ; iFrame.
+  by iIntros "!> [% _]".
+  iIntros (w) "[-> Hf]".
+  iSimpl.
+  rewrite (separate5 (i32const (v + 4 + _ * 4))).
+  iApply wp_seq_ctx.
+  iSplitR ; last first.
+  iSplitL "HΦ Hf Htab Hcl".
+  rewrite (separate2 (i32const (v + 4 + _ * 4))).
+  iApply wp_val_app ; first done.
+  iSplitR ; last first.
+  iApply wp_wand_r ; iSplitL.
+  unfold take ; fold (take (A := value)).
+  rewrite Htail.
+  iDestruct (stackAll_app with "HΦ") as "(HΦ & Hy & _)".
+  rewrite (separate1 _ [_;AI_basic (BI_call_indirect 1)]).
+  rewrite - (app_nil_r [_ ; AI_basic (BI_call_indirect 1)]).
+  iApply wp_wasm_empty_ctx.
+  iApply wp_base_push ; first done.
+  iApply (wp_call_indirect_success_ctx with "Htab Hcl Hf").
+  simpl.
+  unfold cl_type.
+  rewrite Hclt.
+  done.
+  simpl.
+  done.
+  iIntros "!> (Htab & Hcl & Hf)".
+  iApply wp_base_pull.
+  iApply wp_wasm_empty_ctx.
+  simpl.
+  iApply ("Hspec" with "[Hy Hf Htab Hcl]").
+  iFrame.
+  iPureIntro => //=.
+  iIntros (w) "(H & Hf & ?)".
+  iDestruct "H" as (v1) "[-> Hv1]".
+  instantiate (1 := λ x, (∃ v1, ⌜ x = immV _ ⌝ ∗ stackAll ys Φ ∗ Ψ y v1 ∗
+                         N.of_nat j0↦[wt][N.of_nat (Z.to_nat (Wasm_int.Int32.unsigned f))]
+                         Some a ∗
+                         N.of_nat a↦[wf]cl )%I) ;
+    iFrame.
+  iExists  _; by iFrame.
+  iIntros (w) "[H Hf]".
+  iDestruct "H" as (v1) "[-> H]".
+  iSimpl.
+  instantiate (1 := λ x, (∃ v1, ⌜ x = immV _ ⌝ ∗ stackAll ys Φ ∗ Ψ y v1 ∗
+                                           N.of_nat j0↦[wt][N.of_nat (Z.to_nat (Wasm_int.Int32.unsigned f))]
+                                            Some a ∗ N.of_nat a↦[wf]cl
+                                           ∗ ↪[frame] _)%I).
+  iExists _ ; by iFrame.
+  iIntros "!> H".
+  by iDestruct "H" as (v1) "[% _]".
+  iIntros (w) "Hf".
+  iDestruct "Hf" as (v1) "(-> & HΦ & Hv1 & Htab & Hcl & Hf)".
+  iSimpl.
+  rewrite (separate4 (i32const (v + 4 + _ * 4))).
+  iApply wp_seq_ctx.
+  iSplitR ; last first.
+  iSplitL "Hf H".
+  rewrite (separate1 (i32const (v + 4 + _ * 4))).
+  iApply wp_val_app ; first done.
+  iSplitR ; last first.
+  iApply wp_wand_r.
+  iSplitL.
+  iApply wp_store ; last first.
+  simpl.
+  iFrame.
+  iNext.
+  by instantiate (1 := λ x, ⌜ x = immV [] ⌝%I).
+  done.
+  done.
+  done.
+  iIntros (w) "[[-> H] Hf]".
+  iSimpl.
+  by instantiate (1 := λ x, (⌜ x = immV _ ⌝ ∗ N.of_nat n↦[wms][ _ ] _ ∗ ↪[frame] _)%I) ;
+  iFrame.
+  by iIntros "!> [% _]".
+  iIntros (w) "(-> & H & Hf)".
+  iSimpl.
+  rewrite (separate3 (i32const (v + 4 + _ * 4))).
+  iApply wp_seq_ctx.
+  iSplitR ; last first.
+  iSplitL "Hf".
+  iApply (wp_binop with "Hf").
+  done.
+  by instantiate (1 := λ x, ⌜ x = immV _ ⌝%I).
+  iIntros (w) "[-> Hf]".
+  iSimpl.
+  rewrite (separate2 (AI_basic (BI_const (VAL_int32 (Wasm_int.Int32.iadd _ _))))).
+  iApply wp_seq_ctx.
+  iSplitR ; last first.
+  iSplitL "Hf".
+  iApply (wp_set_local with "Hf") => /=.
+  destruct (f_locs f0) ; first done.
+  destruct l ; first done.
+  destruct l ; first by simpl in Hlocs ; lia.
+  destruct l ; first by simpl in Hlocs ; lia.
+  simpl.
+  lia.
+  by instantiate (1 := λ x, x = immV _).
+  iIntros (w) "[-> Hf]".
+  simpl.
+  rewrite set_nth_write.
+  all : try by iIntros "[% _]".
+  all : try by iIntros "Habs" ; iDestruct "Habs" as (?) "[% _]".
+  rewrite - (app_nil_l [AI_basic (BI_br 0)]).
+  iApply (wp_br_ctx_nested with "Hf").
+  lia.
+  done.
+  instantiate (1 := LH_rec [] 0 [] (LH_base [] []) []) => //=.
+  done.
+  done.
+  iIntros "!> Hf".
+  iSimpl.
+  rewrite - (app_nil_l [AI_basic (BI_loop _ _)]).
+  iApply (wp_loop_ctx with "Hf") => //.
+  iIntros "!> Hf".
+  simpl.
+  rewrite - (cat0s (AI_basic (BI_get_local 2) :: _)).
+  rewrite - (cats0 [AI_basic _;_;_;_;_;_;_;_;_;_;_;_;_;_;_]). 
+  iApply wp_label_push ; first done.
+  iApply ("IHj" with "[] [] [Hf] [Hv Hbs Hs' Hs H Hlen Hdiv] [HΦ] [HΨ Hv1] Htab Hcl").
+  iPureIntro.
+  lia.
+  instantiate (1 := v1 :: s').
+  iPureIntro.
+  simpl.
+  rewrite Hs' => //=.
+  lia.
+  unfold Wasm_int.Int32.iadd, Wasm_int.Int32.add.
+  rewrite Wasm_int.Int32.unsigned_repr.
+  rewrite Wasm_int.Int32.unsigned_repr.
+  remember (length s) as x. rewrite - Heqx.
+  replace (v + 4 + (S x - S j) * 4 + 4)%Z
+    with (v + 4 + (S x - j) * 4)%Z.
+  iExact "Hf".
+  lia.
+  lia.
+  lia.
+  unfold isStack.
+  iFrame.
+  iDestruct "Hlen" as "%".
+  iSplit ; first iPureIntro.
+  rewrite app_length.
+  rewrite firstn_length.
+  replace (j `min` length (v0 :: s)) with j ; last by simpl ; lia.
+  simpl.
+  rewrite Hs'.
+  simpl.
+  lia.
+  iSplitL "Hv".
+  rewrite app_length.
+  rewrite firstn_length.
+  simpl.
+  remember (length s) as x. rewrite - Heqx.
+  replace (j `min` S x) with j ; last by simpl ; lia.
+  simpl.
+  rewrite Hs'.
+  simpl.
+  rewrite - Heqx.
+  replace (j + S (x - j)) with (S (x)) ; last lia.
+  iExact "Hv".
+  iSplitR "Hbs".
+  iApply big_sepL_app.
+  iSplitL "Hs".
+  replace j with (j `min` S j) ; last lia.
+  rewrite - take_take.
+  simpl.
+  rewrite Htail.
+  replace j with (length ys).
+  rewrite take_app.
+  iApply (big_sepL_impl with "Hs").
+  iIntros "!>" (k x) "% H".
+  remember (length s) as z ; rewrite - Heqz.
+  replace (S z) with (length (ys ++ v1 :: s')) ; first done.
+  rewrite app_length.
+  simpl.
+  rewrite Hs'.
+  simpl.
+  rewrite - Heqz.
+  remember (length ys) as zz ; rewrite - Heqzz.
+  replace zz with j ; first lia.
+  specialize (f_equal length Htail) as Hl.
+  simpl in Hl.
+  rewrite app_length in Hl ; simpl in Hl.
+  rewrite firstn_length in Hl.
+  subst z. rewrite Hjmin in Hl. rewrite - Heqzz in Hl. lia.
+  specialize (f_equal length Htail) as Hl.
+  simpl in Hl.
+  rewrite app_length in Hl ; simpl in Hl.
+  rewrite firstn_length in Hl.
+  rewrite Hjmin in Hl.
+  remember (length ys) as zz.
+  rewrite - Heqzz in Hl.
+  lia.
+  iSplitL "H".
+  iApply i32_wms.
+  rewrite Wasm_int.Int32.Z_mod_modulus_eq.
+  rewrite Z.mod_small.
+  rewrite N.add_0_r.
+  rewrite Nat.add_0_r.
+  rewrite app_length.
+  rewrite firstn_length.
+  simpl.
+  remember (length s) as x ; rewrite - Heqx.
+  replace (j `min` S x) with j ; last by simpl ; lia.
+  rewrite Hs'.
+  simpl.
+  rewrite - Heqx.
+  replace (j + S (x - j)) with (S (x)) ; last lia.
+  replace (v + 4 + S x *4 - 4 -4 * j)%Z
+    with  (v + 4 + ( S x - S j) * 4)%Z ; last lia.
+  iExact "H".
+  unfold Wasm_int.Int32.max_unsigned in Hv.
+  lia.
+  iApply (big_sepL_impl with "Hs'").
+  iIntros "!>" (k x) "% H".
+  rewrite app_length.
+  rewrite firstn_length.
+  simpl.
+  remember (length s) as z ; rewrite - Heqz.
+  replace (j `min` S z) with j ; last by simpl ; lia.  
+  rewrite Hs'.
+  simpl.
+  rewrite - Heqz.
+  replace (j + S (z - j)) with (S z) ; last lia.
+  replace (S ( j + k)) with (j + S k) ; last lia.
+  iExact "H".
+  iDestruct "Hbs" as (bs) "[% H]".
+  iExists bs.
+  iSplit ; first iPureIntro.
+  rewrite app_length.
+  rewrite firstn_length.
+  simpl.
+  remember (length s) as x ; rewrite - Heqx.
+  replace (j `min` S x) with j ; last by simpl ; lia.
+  simpl.
+  rewrite Hs'.
+  simpl.
+  lia.
+  rewrite app_length.
+  rewrite firstn_length.
+  simpl.
+  remember (length s) as x ; rewrite - Heqx.
+  replace (j `min` S x) with j ; last by simpl ; lia.
+  simpl.
+  rewrite Hs'.
+  simpl.
+  rewrite - Heqx.
+  replace (j + S (x - j)) with (S x) ; last lia.
+  iExact "H".
+  replace j with (j `min` S j) ; last lia.
+  rewrite - take_take.
+  simpl.
+  rewrite Htail.
+  replace j with (length ys).
+  rewrite take_app.
+  done.
+  specialize (f_equal length Htail) as Hl.
+  simpl in Hl.
+  rewrite app_length in Hl ; simpl in Hl.
+  rewrite firstn_length in Hl.
+  rewrite Hjmin in Hl.
+  remember (length ys) as zz ; rewrite - Heqzz in Hl ;
+    lia.
+  rewrite - (take_drop j s).
+  rewrite app_comm_cons.
+  rewrite Htail.
+  rewrite take_drop.
+  rewrite drop_app_le.
+  replace j with (length ys).
+  rewrite drop_app.
+  simpl.
+  iFrame.
+  specialize (f_equal length Htail) as Hl.
+  simpl in Hl.
+  rewrite app_length in Hl ; simpl in Hl.
+  rewrite firstn_length in Hl.
+   rewrite Hjmin in Hl.
+  remember (length ys) as zz ; rewrite - Heqzz in Hl ;
+    lia.
+  specialize (f_equal length Htail) as Hl.
+  simpl in Hl.
+  rewrite app_length in Hl ; simpl in Hl.
+  rewrite firstn_length in Hl.
+  rewrite app_length.
+  rewrite - Hl.
+  lia.
+  iExact "HΞ". }
+  iApply ("H" with "[] [] [Hf] [Hn Hs] [HΦ] [] Htab Hcl").
+  instantiate (1 := length s).
+  iPureIntro ; lia.
+  instantiate (1 := []).
+  iPureIntro ; simpl ; lia.
+  rewrite Z.sub_diag.
+  rewrite Z.mul_0_l.
+  rewrite Z.add_0_r.
+  done.
+  iDestruct "Hs" as "(% & % & Hs & Hbs)".
+  iSplit ; first done.
+  iSplit ; first iPureIntro.
+  rewrite cats0 firstn_length.
+  rewrite Nat.min_id.
+  exact H0.
+  iSplitL "Hn".
+  iApply i32_wms.
+  rewrite N.add_0_r.
+  rewrite Wasm_int.Int32.Z_mod_modulus_eq.
+  rewrite Z.mod_small.
+  rewrite cats0 firstn_length.
+  rewrite Nat.min_id.
+  done.
+  unfold Wasm_int.Int32.max_unsigned in Hv ; lia.
+  iSplitL "Hs".
+  rewrite cats0 firstn_length.
+  rewrite firstn_all.
+  rewrite Nat.min_id.
+  done.
+  rewrite cats0 firstn_length.
+  rewrite Nat.min_id.
+  done.
+  rewrite firstn_all.
+  done.
+  rewrite drop_all.
+  done.
+  done.
+  all : try by iIntros "[% _]".
+  by iIntros "[[[% _] _] _]".
+Qed.
+          
                                         
     
     
@@ -2056,7 +2966,8 @@ Section Client.
      1 - is_empty
      2 - is_full
      3 - pop
-     4 - push *)
+     4 - push 
+     5 - map *)
   Definition main :=
     [ AI_basic (BI_call 0) ;
       AI_basic (BI_tee_local 0) ;
@@ -2070,6 +2981,9 @@ Section Client.
       i32const 6 ;
       AI_basic (BI_get_local 0) ;
       AI_basic (BI_call 4) ;
+      i32const 0 ;
+      AI_basic (BI_get_local 0) ;
+      AI_basic (BI_call 5) ;
       AI_basic (BI_get_local 0) ;
       AI_basic (BI_call 3) ;
       AI_basic (BI_get_local 0) ;
@@ -2077,6 +2991,11 @@ Section Client.
       AI_basic (BI_binop T_i32 (Binop_i BOI_sub)) ;
       AI_basic (BI_set_global 0)
     ].
+
+  Definition square :=
+    [ AI_basic (BI_get_local 0) ;
+      AI_basic (BI_get_local 0) ;
+      AI_basic (BI_binop T_i32 (Binop_i BOI_mul)) ].
 
   Fixpoint basic_expr_of_expr es :=
     match es with
@@ -2100,7 +3019,7 @@ Section Client.
       mod_types := [
         Tf [] [T_i32] ;
         Tf [T_i32] [T_i32] ;
-        Tf [T_i32 ; T_i32] []
+        Tf [T_i32 ; T_i32] [] 
       ] ;
       mod_funcs := [
         {|
@@ -2127,9 +3046,15 @@ Section Client.
           modfunc_type := Mk_typeidx 2 ;
           modfunc_locals := [T_i32] ;
           modfunc_body := mk_basic_expr push
+        |} ;
+        {|
+          modfunc_type := Mk_typeidx 2 ;
+          modfunc_locals := [T_i32 ; T_i32] ;
+          modfunc_body := mk_basic_expr stack_map
         |}
       ] ;
-      mod_tables := [] ;
+      mod_tables := [ {| modtab_type := {| tt_limits := {| lim_min := 2%N ; lim_max := None |} ;
+                                        tt_elem_type := ELT_funcref |} |} ] ;
       mod_mems := [
         {| lim_min := 0%N ; lim_max := None |}
       ] ;
@@ -2158,6 +3083,14 @@ Section Client.
         {|
           modexp_name := list_byte_of_string "push" ;
           modexp_desc := MED_func (Mk_funcidx 4)
+        |} ;
+        {|
+          modexp_name := list_byte_of_string "stack_map" ;
+          modexp_desc := MED_func (Mk_funcidx 5)
+        |} ;
+        {|
+          modexp_name := list_byte_of_string "table" ;
+          modexp_desc := MED_table (Mk_tableidx 0)
         |}
       ]
     |}.
@@ -2170,15 +3103,23 @@ Section Client.
           modfunc_type := Mk_typeidx 0 ;
           modfunc_locals := [T_i32] ;
           modfunc_body := mk_basic_expr main
-        |} ] ;
-      mod_tables := [] ;
+        |} ;
+                     {|
+                       modfunc_type := Mk_typeidx 2 ;
+                       modfunc_locals := [] ;
+                       modfunc_body := mk_basic_expr square
+                     |} ] ;
+      mod_tables := [] ; (* {| modtab_type := {| tt_limits := {| lim_min := 0%N ; lim_max := None |} ;
+                                        tt_elem_type := ELT_funcref |} |} ] ; *)
       mod_mems := [] ;
       mod_globals := [ {| modglob_type := {| tg_t := T_i32 ;
                                             tg_mut := MUT_mut |} ;
                          modglob_init := [bi32const 0] |} ] ;
-      mod_elem := [] ;
+      mod_elem := [ {| modelem_table := Mk_tableidx 0 ;
+                      modelem_offset := [bi32const 0] ;
+                      modelem_init := [Mk_funcidx 7] |} ] ;
       mod_data := [] ;
-      mod_start := Some {| modstart_func := Mk_funcidx 5 |} ;
+      mod_start := Some {| modstart_func := Mk_funcidx 6 |} ;
       mod_imports := [
         {|
           imp_module := list_byte_of_string "Stack" ;
@@ -2204,7 +3145,15 @@ Section Client.
           imp_module := list_byte_of_string "Stack" ;
           imp_name := list_byte_of_string "push" ;
           imp_desc := ID_func 3
-        |}
+        |} ;
+        {| imp_module := list_byte_of_string "Stack" ;
+          imp_name := list_byte_of_string "stack_map" ;
+          imp_desc := ID_func 3
+        |} ;
+        {| imp_module := list_byte_of_string "Stack" ;
+          imp_name := list_byte_of_string "table" ;
+          imp_desc := ID_table {| tt_limits := {| lim_min := 2%N ; lim_max := None |} ;
+                                 tt_elem_type := ELT_funcref |} |}
       ] ;
       mod_exports := [
         {|
@@ -2217,7 +3166,9 @@ Section Client.
 
   Definition expts := [ET_func (Tf [] [T_i32]) ; ET_func (Tf [T_i32] [T_i32]);
                    ET_func (Tf [T_i32] [T_i32]) ; ET_func (Tf [T_i32] [T_i32]);
-                   ET_func (Tf [T_i32 ; T_i32] [])].
+                       ET_func (Tf [T_i32 ; T_i32] []) ; ET_func (Tf [T_i32 ; T_i32] []) ;
+                       ET_tab {| tt_limits := {| lim_min := 2%N ; lim_max := None |} ;
+                                tt_elem_type := ELT_funcref |} ].
 
   Ltac bet_first f :=
     eapply bet_composition_front ; first eapply f => //=.
@@ -2227,7 +3178,7 @@ Section Client.
   Proof.
     unfold module_typing => /=. 
     exists [Tf [] [T_i32] ; Tf [T_i32] [T_i32] ; Tf [T_i32] [T_i32] ;
-       Tf [T_i32] [T_i32] ; Tf [T_i32 ; T_i32] [] ], [].
+       Tf [T_i32] [T_i32] ; Tf [T_i32 ; T_i32] [] ; Tf [T_i32 ; T_i32] [] ], [].
     repeat split => //.
     repeat (apply Forall2_cons ; repeat split => //) => /=.
     - bet_first bet_const.
@@ -2357,21 +3308,76 @@ Section Client.
       apply bet_binop.
       apply Binop_i32_agree.
       apply bet_store => //.
+    - bet_first bet_get_local.
+      bet_first bet_load.
+      bet_first bet_set_local.
+      bet_first bet_get_local.
+      eapply bet_composition_front.
+      rewrite (separate1 T_i32).
+      apply bet_weakening.
+      apply bet_const.
+      bet_first bet_binop.
+      apply Binop_i32_agree.
+      bet_first bet_set_local.
+      apply bet_block.
+      apply bet_loop => /=.
+      bet_first bet_get_local.
+      eapply bet_composition_front.
+      rewrite (separate1 T_i32).
+      apply bet_weakening.
+      apply bet_get_local => //.
+      bet_first bet_relop.
+      apply Relop_i32_agree.
+      rewrite - (app_nil_l [T_i32]).
+      bet_first bet_br_if.
+      bet_first bet_get_local.
+      eapply bet_composition_front.
+      rewrite (separate1 T_i32).
+      apply bet_weakening.
+      apply bet_get_local => //.
+      eapply bet_composition_front.
+      simpl ; rewrite (separate2 T_i32).
+      apply bet_weakening.
+      apply bet_get_local => //.
+      eapply bet_composition_front.
+      simpl ; rewrite (separate2 T_i32 _ [_]).
+      apply bet_weakening.
+      apply bet_load => //.
+      eapply bet_composition_front.
+      simpl ; rewrite (separate3 T_i32 T_i32 T_i32 []).
+      apply bet_weakening.
+      apply bet_get_local => //.
+      eapply bet_composition_front.
+      simpl ; rewrite (separate2 T_i32 T_i32 [_;_]).
+      apply bet_weakening.
+      rewrite (separate1 T_i32 [_]).
+      apply bet_call_indirect => //=.
+      eapply bet_composition_front.
+      simpl ; rewrite (separate1 T_i32 [_;_]).
+      apply bet_weakening.
+      apply bet_store => //.
+      eapply bet_composition_front.
+      apply bet_weakening.
+      apply bet_const.
+      bet_first bet_binop.
+      apply Binop_i32_agree.
+      bet_first bet_set_local.
+      rewrite - (app_nil_l []).
+      apply bet_br => //. 
     - unfold module_export_typing.
       repeat (apply Forall2_cons ; repeat split => //) => //=.
   Qed.
-  Print expts.
+
 
   Lemma module_typing_client :
     module_typing client_module expts [ET_glob {| tg_t := T_i32 ; tg_mut := MUT_mut |} ].
   Proof.
     unfold module_typing => /=.
-    exists [ Tf [] [] ],
+    exists [ Tf [] [] ; Tf [T_i32] [T_i32] ],
       [ {| tg_t := T_i32 ; tg_mut := MUT_mut |} ].
     repeat split => //.
-    - apply Forall2_cons.
-      repeat split => //=.
-      bet_first bet_call.
+    repeat (apply Forall2_cons ; repeat split => //) => /=.
+    - bet_first bet_call.
       bet_first bet_tee_local.
       eapply bet_composition_front.
       rewrite (separate1 T_i32 []).
@@ -2398,6 +3404,12 @@ Section Client.
       apply bet_weakening.
       by apply bet_get_local.
       bet_first bet_call.
+      bet_first bet_const.
+      eapply bet_composition_front.
+      rewrite (separate1 T_i32 []).
+      apply bet_weakening.
+      by apply bet_get_local.
+      bet_first bet_call.
       bet_first bet_get_local.
       bet_first bet_call.
       eapply bet_composition_front.
@@ -2410,9 +3422,20 @@ Section Client.
       bet_first bet_binop.
       apply Binop_i32_agree.
       by eapply bet_set_global.
+    - bet_first bet_get_local.
+      eapply bet_composition_front.
+      rewrite (separate1 T_i32 []).
+      apply bet_weakening.
+      by apply bet_get_local.
+      apply bet_binop.
+      apply Binop_i32_agree.
     - apply Forall2_cons.
       repeat split => //.
       by apply bet_const.
+    - unfold module_elem_typing.
+      apply Forall_cons.
+      repeat split => //.
+      apply bet_const.
     - unfold module_import_typing.
       repeat (apply Forall2_cons ; repeat split => //) => //=.
     - apply Forall2_cons.
@@ -2421,8 +3444,8 @@ Section Client.
 
   Definition module_decls := [ stack_module ; client_module ].
   Definition stack_instantiate :=
-    [ ID_instantiate [0%N ; 1%N ; 2%N ; 3%N ; 4%N] 0 [] ;
-      ID_instantiate [5%N] 1 [0%N ; 1%N ; 2%N ; 3%N ; 4%N] ].
+    [ ID_instantiate [0%N ; 1%N ; 2%N ; 3%N ; 4%N ; 5%N ; 6%N] 0 [] ;
+      ID_instantiate [7%N] 1 [0%N ; 1%N ; 2%N ; 3%N ; 4%N ; 5%N ; 6%N] ].
 
   Notation " n ↪[vis]{ q } v" := (ghost_map_elem (V := module_export) visGName n q v%V)
                            (at level 20, q at level 5, format " n ↪[vis]{ q } v") .
@@ -2434,32 +3457,32 @@ Section Client.
   Notation " n ↪[mods] v" := (ghost_map_elem (V := module) msGName n (DfracOwn 1) v%V)
                                (at level 20, format " n ↪[mods] v").
 
-  Notation "{{{ P }}} es {{{ v , Q }}}" :=
-  (□ ∀ Φ, P -∗ (∀ v, Q -∗ Φ v) -∗ WP es @ NotStuck ; ⊤ (*CTX_EMPTY*) {{ v, Φ v }})%I (at level 50). 
+(*  Notation "{{{ P }}} es {{{ v , Q }}}" :=
+  (□ ∀ Φ, P -∗ (∀ v, Q -∗ Φ v) -∗ WP es @ NotStuck ; ⊤ (*CTX_EMPTY*) {{ v, Φ v }})%I (at level 50). *)
 
  Context `{!wfuncG Σ, !wtabG Σ, !wtabsizeG Σ, !wmemG Σ, !wmemsizeG Σ, !wglobG Σ, !wframeG Σ, !hvisG Σ, !hmsG Σ,  !logrel_na_invs Σ}.
 
-  Definition stack_instance idfs m :=
+  Definition stack_instance idfs m t :=
     {|
       inst_types := [Tf [] [T_i32] ; Tf [T_i32] [T_i32] ; Tf [T_i32 ; T_i32] []] ;
       inst_funcs := idfs ;
-      inst_tab := [] ;
+      inst_tab := [t] ;
       inst_memory := [m] ;
       inst_globs := []
     |}.
 
 
-  Definition finst (f : function_closure) :=
+(*   Definition finst (f : function_closure) :=
     match f with
     | FC_func_native inst _ _ _ => Some inst
-    | _ => None end.
+    | _ => None end. *)
 
 (*  Class logrel_na_invs Σ :=
   {
     logrel_na_invG :> na_invG Σ;
     logrel_nais : na_inv_pool_name;
   }. *)
-
+(*
 Definition wf : string := "wfN".
 Definition wf0 : string := "wf0N".
 Definition wf1 : string := "wf1N".
@@ -2471,9 +3494,9 @@ Definition wf0N : namespace := nroot .@ wf0.
 Definition wf1N : namespace := nroot .@ wf1.
 Definition wf2N : namespace := nroot .@ wf2.
 Definition wf3N : namespace := nroot .@ wf3.
-Definition wlenN : namespace := nroot .@ wlen.
+Definition wlenN : namespace := nroot .@ wlen. *)
 
-Definition spec0 idf0 i0 l0 f0 (isStack : Z -> seq.seq value -> iPropI Σ)  nextStackAddrIs :=
+Definition spec0 idf0 i0 l0 f0 (isStack : Z -> seq.seq i32 -> iPropI Σ)  nextStackAddrIs :=
   (∀ f addr, {{{ ↪[frame] f ∗
                   N.of_nat idf0 ↦[wf] FC_func_native i0 (Tf [] [T_i32]) l0 f0 ∗
                   nextStackAddrIs addr ∗
@@ -2490,7 +3513,7 @@ Definition spec0 idf0 i0 l0 f0 (isStack : Z -> seq.seq value -> iPropI Σ)  next
                                                                                                                                              N.of_nat idf0 ↦[wf] FC_func_native i0 (Tf [] [T_i32]) l0 f0 ∗
                                                                                                                                              ↪[frame] f }}} )%I.
 
-Definition spec1 idf1 i1 l1 f1 (isStack : Z -> seq.seq value -> iPropI Σ) :=
+Definition spec1 idf1 i1 l1 f1 (isStack : Z -> seq.seq i32 -> iPropI Σ) :=
   (∀ v s f, {{{ ↪[frame] f  ∗
                  N.of_nat idf1 ↦[wf] FC_func_native i1 (Tf [T_i32] [T_i32]) l1 f1 ∗
                  ⌜ (0 <= v <= Wasm_int.Int32.max_unsigned - 4 - length s * 4)%Z ⌝ ∗ 
@@ -2502,7 +3525,7 @@ Definition spec1 idf1 i1 l1 f1 (isStack : Z -> seq.seq value -> iPropI Σ) :=
                                                  N.of_nat idf1 ↦[wf] FC_func_native i1 (Tf [T_i32] [T_i32]) l1 f1 ∗ 
                                                  ↪[frame] f}}})%I.
 
-Definition spec2 idf2 i2 l2 f2 (isStack : Z -> seq.seq value -> iPropI Σ) :=
+Definition spec2 idf2 i2 l2 f2 (isStack : Z -> seq.seq i32 -> iPropI Σ) :=
   (∀ v s f, {{{ ↪[frame] f ∗
                  N.of_nat idf2 ↦[wf] FC_func_native i2 (Tf [T_i32] [T_i32]) l2 f2 ∗
                  ⌜ (0 <= v <= Wasm_int.Int32.max_unsigned - 4 - length s * 4 )%Z ⌝ ∗ 
@@ -2514,14 +3537,13 @@ Definition spec2 idf2 i2 l2 f2 (isStack : Z -> seq.seq value -> iPropI Σ) :=
                                                                             N.of_nat idf2 ↦[wf] FC_func_native i2 (Tf [T_i32] [T_i32]) l2 f2 ∗ 
                                                                             ↪[frame] f }}})%I.
 
-Definition spec3 idf3 i3 l3 f3 (isStack : Z -> seq.seq value -> iPropI Σ) :=
+Definition spec3 idf3 i3 l3 f3 (isStack : Z -> seq.seq i32 -> iPropI Σ) :=
   (∀ a v s f, {{{ ↪[frame] f ∗
                    N.of_nat idf3 ↦[wf] FC_func_native i3 (Tf [T_i32] [T_i32]) l3 f3
                    ∗ ⌜ (0 <= v <= Wasm_int.Int32.max_unsigned - 4 - S (length s) * 4 )%Z ⌝
-                   ∗ ⌜ types_agree T_i32 a ⌝
                    ∗ isStack v (a :: s) }}}
                 [i32const v ; AI_invoke idf3]
-                {{{ w, ⌜ w = immV [a] ⌝ ∗
+                {{{ w, ⌜ w = immV [VAL_int32 a] ⌝ ∗
                                   isStack v s ∗
                                   N.of_nat idf3 ↦[wf] FC_func_native i3 (Tf [T_i32] [T_i32]) l3 f3 ∗
                                   ↪[frame] f }}})%I.
@@ -2530,31 +3552,70 @@ Definition spec4 idf4 i4 l4 f4 isStack :=
   (∀ a v s f, {{{ ↪[frame] f ∗
                    N.of_nat idf4 ↦[wf] FC_func_native i4 (Tf [T_i32 ; T_i32] []) l4 f4 
                    ∗ ⌜ (0 <= v <= Wasm_int.Int32.max_unsigned - 4 - S (length s) * 4 )%Z ⌝
-                   ∗ ⌜ types_agree T_i32 a ⌝
                    ∗ ⌜ (length s < two14 - 1)%Z ⌝
                    ∗ isStack v s }}}
-                [ AI_basic (BI_const a) ; i32const v ; AI_invoke idf4 ]
+                [ AI_basic (BI_const (VAL_int32 a)) ; i32const v ; AI_invoke idf4 ]
                 {{{ w, ⌜ w = immV [] ⌝ ∗
                                   isStack v (a :: s) ∗
                                   N.of_nat idf4 ↦[wf] FC_func_native i4 (Tf [T_i32 ; T_i32] []) l4 f4 ∗
                                   ↪[frame] f }}})%I.
 
-  Lemma instantiate_stack_spec (s : stuckness) E hv0 hv1 hv2 hv3 hv4 :
-    (* Knowing 0%N holds the stack module… *)
-    0%N ↪[mods] stack_module -∗
+Definition spec5 idf5 i5 l5 f5 (isStack : Z -> seq.seq i32 -> iPropI Σ) j0 :=
+  (∀ (f0 : frame) (f : i32) (v : Z) (s : seq.seq i32) a cl
+      (Φ : i32 -> iPropI Σ) (Ψ : i32 -> i32 -> iPropI Σ) ,
+      {{{  ↪[frame] f0 ∗
+            N.of_nat idf5 ↦[wf] FC_func_native i5 (Tf [T_i32 ; T_i32] []) l5 f5 ∗
+            ⌜ (0 <= v)%Z ⌝ ∗
+            ⌜ (v + 4 + length s * 4 ≤ Wasm_int.Int32.max_unsigned)%Z ⌝ ∗
+            isStack v s ∗
+            stackAll s Φ ∗
+            N.of_nat j0 ↦[wt][ N.of_nat (Wasm_int.nat_of_uint i32m f) ] (Some a) ∗
+            (N.of_nat a) ↦[wf] cl ∗
+            ⌜ match cl with FC_func_native _ t _ _ => t | FC_func_host t _ => t end
+         = Tf [T_i32] [T_i32] ⌝ ∗ 
+              (∀ (u : i32) (fc : frame),
+                   {{{ Φ u ∗
+                      ⌜ i5 = f_inst fc ⌝ ∗
+                       ↪[frame] fc ∗
+                       N.of_nat j0 ↦[wt][ N.of_nat (Wasm_int.nat_of_uint i32m f) ] (Some a) ∗
+                       (N.of_nat a) ↦[wf] cl
+                  }}}
+                  [ AI_basic (BI_const (VAL_int32 u)) ;
+                    AI_invoke a ]
+                  {{{ w, (∃ v, ⌜ w = immV [VAL_int32 v] ⌝ ∗ Ψ u v)
+                           ∗ ↪[frame] fc
+                           ∗ N.of_nat j0 ↦[wt][ N.of_nat (Wasm_int.nat_of_uint i32m f) ] (Some a) 
+                           ∗ (N.of_nat a) ↦[wf] cl }}}
+                  )  }}}
+    [ AI_basic (BI_const (VAL_int32 f)) ; i32const v ; AI_invoke idf5 ]
+    {{{ w, ⌜ w = immV [] ⌝ ∗
+           (∃ s', isStack v s' ∗ stackAll2 s s' Ψ) ∗
+           N.of_nat idf5 ↦[wf] FC_func_native i5 (Tf [T_i32 ; T_i32] []) l5 f5 ∗
+           ↪[frame] f0
+    }}})%I.
+
+
+Lemma instantiate_stack_spec (s : stuckness) E (hv0 hv1 hv2 hv3 hv4 hv5 hv6 : module_export) :
+  (* Knowing 0%N holds the stack module… *)
+  0%N ↪[mods] stack_module -∗
      (* … and we own the vis 0%N thru 4%N … *)
-     ([∗ list] k↦hvk ∈ [hv0 ; hv1 ; hv2 ; hv3 ; hv4], N.of_nat k ↪[vis] hvk) -∗
+     ([∗ list] k↦hvk ∈ [hv0 ; hv1 ; hv2 ; hv3 ; hv4 ; hv5 ; hv6], N.of_nat k ↪[vis] hvk) -∗
      (* … instantiating the stack-module (by lazyness, this is expressed here with
         a take 1 in order to avoir rewriting the instantiation), yields the following : *)
      WP ((take 1 stack_instantiate, []) : host_expr)
      @ s ; E
              {{ v,
+                    
                  (* 0%N still owns the stack_module *)
-                 0%N ↪[mods] stack_module ∗
-                  ∃ idf0 idf1 idf2 idf3 idf4 name0 name1 name2 name3 name4
-                    f0 f1 f2 f3 f4 i0 i1 i2 i3 i4 l0 l1 l2 l3 l4
-                    (isStack : Z -> seq.seq value -> iPropI Σ)
-                    nextStackAddrIs,
+                 0%N ↪[mods] stack_module ∗ 
+                  ∃ (idf0 idf1 idf2 idf3 idf4 idf5 idt : nat)
+                    (name0 name1 name2 name3 name4 name5 name6 : name)
+                    (f0 f1 f2 f3 f4 f5 : list basic_instruction)
+                    (i0 i1 i2 i3 i4 i5 : instance)
+                    (l0 l1 l2 l3 l4 l5 : list value_type)
+                    tab 
+                    (isStack : Z -> seq.seq i32 -> iPropI Σ)
+                    (nextStackAddrIs : nat -> iPropI Σ), 
                     (* Our exports are in the vis 0%N thru 4%N. Note that everything is 
                        existantially quantified. In fact, all the f_i, i_i and l_i 
                        could be given explicitely, but we quantify them existantially 
@@ -2562,48 +3623,64 @@ Definition spec4 idf4 i4 l4 f4 isStack :=
                        we only care about their spec (see next comment). This also
                        makes this lemma more readable than if we stated explicitely all
                        the codes of the functions *)
-                    let inst_vis := map (λ '(name, idf),
+                    let inst_vis := (map (λ '(name, idf),
                                                  {| modexp_name := name ;
                                                    modexp_desc := MED_func (Mk_funcidx idf)
                                                  |}) [(name0, idf0) ; (name1, idf1) ;
                                                       (name2, idf2) ; (name3, idf3) ;
-                                                      (name4, idf4)] in
+                                                      (name4, idf4) ; (name5, idf5) ])
+                                        ++ [ {| modexp_name := name6 ;
+                                               modexp_desc := MED_table (Mk_tableidx idt) |} ]
+                    in 
                     let inst_map := fold_left (λ fs '(idf,i,t,l,f),
-                                                <[ idf := FC_func_native i t l f ]> fs)
+                                                <[ N.of_nat idf := FC_func_native i t l f ]> fs)
                                               (rev [(idf0, i0, Tf [] [T_i32], l0, f0) ;
                                                (idf1, i1, Tf [T_i32] [T_i32], l1, f1) ;
                                                     (idf2, i2, Tf [T_i32] [T_i32], l2, f2) ;
                                                     (idf3, i3, Tf [T_i32] [T_i32], l3, f3) ;
-                                                    (idf4, i4, Tf [T_i32 ; T_i32] [], l4, f4)])
-                                              ∅ in
+                                                    (idf4, i4, Tf [T_i32 ; T_i32] [], l4, f4) ;
+                                              (idf5, i5, Tf [T_i32 ; T_i32] [], l5, f5)])
+                                              ∅ in 
                     (* These two import functions state that all [vis] and [wf] point 
                        to the correct exports/functions, i.e. a client will be able 
                        to successfully import them *)
-                    import_resources_host [0%N; 1%N; 2%N; 3%N; 4%N] inst_vis ∗
-                                          import_resources_wasm_typecheck inst_vis expts inst_map ∅ ∅ ∅ ∗
-                                          (* We own a token that hides ressources needed for the new_stack function *)
-                                          nextStackAddrIs 0 ∗
-                                          (* And finally we have specs for all our exports : *)
-                                          (* Spec for new_stack (call 0) *)
-                                          spec0 idf0 i0 l0 f0 isStack nextStackAddrIs ∗
-                                          (* Spec for is_empty (call 1) *)
-                                          spec1 idf1 i1 l1 f1 isStack ∗
-                                          (* Spec for is_full (call 2) *)
-                                          spec2 idf2 i2 l2 f2 isStack ∗
-                                          (* Spec for pop (call 3) *)
-                                          spec3 idf3 i3 l3 f3 isStack ∗
-                                          (* Spec for push (call 4) *)
-                                          spec4 idf4 i4 l4 f4 isStack
+                    import_resources_host [0%N; 1%N; 2%N; 3%N; 4%N ; 5%N ; 6%N] inst_vis ∗
+                    import_resources_wasm_typecheck inst_vis expts inst_map
+                    (<[ N.of_nat idt := tab ]> ∅) 
+                    ∅ ∅ ∗
+                    ⌜ length tab.(table_data) > 1 ⌝ ∗ 
+                    (* We own a token that hides ressources needed for the new_stack function *)
+                    nextStackAddrIs 0 ∗
+                    (* And finally we have specs for all our exports : *)
+                    (* Spec for new_stack (call 0) *)
+                    spec0 idf0 i0 l0 f0 isStack nextStackAddrIs ∗
+                    (* Spec for is_empty (call 1) *)
+                    spec1 idf1 i1 l1 f1 isStack ∗
+                    (* Spec for is_full (call 2) *)
+                    spec2 idf2 i2 l2 f2 isStack ∗
+                    (* Spec for pop (call 3) *)
+                    spec3 idf3 i3 l3 f3 isStack ∗
+                    (* Spec for push (call 4) *)
+                    spec4 idf4 i4 l4 f4 isStack ∗
+                    (* Spec of stack_map (call 5) *)
+                    spec5 idf5 i5 l5 f5 isStack idt
                                           
              }}.
   Proof.
-    iIntros "Hmod (Hhv0 & Hhv1 & Hhv2 & Hhv3 & Hhv4 & _)".
-    iApply (weakestpre.wp_strong_mono s _ E with "[Hmod Hhv0 Hhv1 Hhv2 Hhv3 Hhv4]") => //.
-    iApply (instantiation_spec_operational_no_start with "[Hmod Hhv0 Hhv1 Hhv2 Hhv3 Hhv4]") ;
+    iIntros "Hmod (Hhv0 & Hhv1 & Hhv2 & Hhv3 & Hhv4 & Hhv5 & Hhv6 & _)".
+    iApply (weakestpre.wp_strong_mono s _ E
+             with "[Hmod Hhv0 Hhv1 Hhv2 Hhv3 Hhv4 Hhv5 Hhv6]") => //.
+    iApply (instantiation_spec_operational_no_start
+             with "[Hmod Hhv0 Hhv1 Hhv2 Hhv3 Hhv4 Hhv5 Hhv6]") ;
       try exact module_typing_stack => //.
     - by unfold stack_module.
+    - unfold module_restrictions => /=.
+      repeat split => //=.
+      exists [] => //.
+      exists [] => //.
+      exists [] => //.
     - unfold instantiation_resources_pre.
-      iFrame.
+      iSplitL "Hmod" ; first done.
       repeat iSplit.
     - by unfold import_resources_host.
     - iPureIntro. apply dom_empty.
@@ -2624,9 +3701,22 @@ Definition spec4 idf4 i4 l4 f4 isStack :=
       by iExists _.
       iSplitL "Hhv4".
       by iExists _.
+      iSplitL "Hhv5".
+      by iExists _.
+      iSplitL "Hhv6".
+      by iExists _.
+      done.
+      done.
+      iPureIntro.
+      unfold module_elem_bound_check_gmap.
+      simpl.
+      done.
+      iPureIntro.
+      unfold module_data_bound_check_gmap.
+      simpl.
       done.
     - iIntros (v) "(Hmod & Himphost & Himpwasm & Hinst)".
-      iDestruct "Hinst" as (inst g_inits) "(%Hinst & Hexpwasm & Hexphost)".
+      iDestruct "Hinst" as (inst g_inits t_inits m_inits) "(%Hinst & %Hival & Hexpwasm & Hexphost)".
       destruct Hinst as (Hinsttype & Hinstfunc & Hinsttab & Hinstmem & Hinstglob).
       unfold module_inst_resources_wasm, module_export_resources_host => /=.
       destruct inst => /=.
@@ -2644,36 +3734,51 @@ Definition spec4 idf4 i4 l4 f4 isStack :=
         iDestruct "Hexpwf" as "[Hf2 Hexpwf]".
       destruct inst_funcs as [|? inst_funcs] ; first done ;
         iDestruct "Hexpwf" as "[Hf3 Hexpwf]".
+      destruct inst_funcs as [| ? inst_funcs] ; first done ;
+        iDestruct "Hexpwf" as "[Hf4 Hexpwf]".
       destruct inst_funcs ; last done.
+      destruct inst_tab ; first done.
+      iDestruct "Hexpwt" as "[Htab Hexpwt]".
       destruct inst_tab ; last done.
       destruct inst_memory as [|m inst_memory] ; first done.
       iDestruct "Hexpwm" as "[Hexpwm ?]".
       destruct inst_memory ; last done.
       iDestruct "Hexpwm" as "(Hexpwm & Hmemlength & Hmemlim)".
       destruct inst_globs ; last done.
-      iDestruct "Hexphost" as "(Hexp0 & Hexp1 & Hexp2 & Hexp3 & Hexp4 & _)".
+      iDestruct "Hexphost" as "(Hexp0 & Hexp1 & Hexp2 & Hexp3 & Hexp4 & Hexp5 & Hexp6 & _)".
       iDestruct "Hexp0" as (name0) "Hexp0".
       iDestruct "Hexp1" as (name1) "Hexp1".
       iDestruct "Hexp2" as (name2) "Hexp2".
       iDestruct "Hexp3" as (name3) "Hexp3".
       iDestruct "Hexp4" as (name4) "Hexp4".
+      iDestruct "Hexp5" as (name5) "Hexp5".
+      iDestruct "Hexp6" as (name6) "Hexp6".
       simpl in * ; subst.
       iSplitL "Hmod" ; first done.
-      iExists f, f0, f1, f2, f3.
-      iExists name0, name1, name2, name3, name4.
-      do 3 iExists _, _, _, _, _.
+      iExists f, f0, f1, f2, f3, f4, t.
+      iExists name0, name1, name2, name3, name4, name5, name6.
+      do 3 iExists _, _, _, _, _, _.
+      iExists _.
       iExists (λ a b, isStack a b m).
       iExists (λ n, (N.of_nat m↦[wmlength] N.of_nat n)%I).
       iDestruct (mapsto_frac_ne with "Hf Hf0") as "%H01" ; first by eauto.
       iDestruct (mapsto_frac_ne with "Hf Hf1") as "%H02" ; first by eauto.
       iDestruct (mapsto_frac_ne with "Hf Hf2") as "%H03" ; first by eauto.
       iDestruct (mapsto_frac_ne with "Hf Hf3") as "%H04" ; first by eauto.
+      iDestruct (mapsto_frac_ne with "Hf Hf4") as "%H05" ; first by eauto.
       iDestruct (mapsto_frac_ne with "Hf0 Hf1") as "%H12" ; first by eauto.
       iDestruct (mapsto_frac_ne with "Hf0 Hf2") as "%H13" ; first by eauto.
       iDestruct (mapsto_frac_ne with "Hf0 Hf3") as "%H14" ; first by eauto.
+      iDestruct (mapsto_frac_ne with "Hf0 Hf4") as "%H15" ; first by eauto.
       iDestruct (mapsto_frac_ne with "Hf1 Hf2") as "%H23" ; first by eauto.
       iDestruct (mapsto_frac_ne with "Hf1 Hf3") as "%H24" ; first by eauto.
+      iDestruct (mapsto_frac_ne with "Hf1 Hf4") as "%H25" ; first by eauto.
       iDestruct (mapsto_frac_ne with "Hf2 Hf3") as "%H34" ; first by eauto.
+      iDestruct (mapsto_frac_ne with "Hf2 Hf4") as "%H35" ; first by eauto.
+      iDestruct (mapsto_frac_ne with "Hf3 Hf4") as "%H45" ; first by eauto.
+      (*  assert (forall a b, N.of_nat a <> N.of_nat b -> a <> b) as Hneq.
+      { intros ; intro. by subst. }
+      apply Hneq in H01, H02, H03, H04, H05, H12, H13, H14, H15, H23, H24, H25, H34, H35, H45. *)
 (*      iMod (na_inv_alloc logrel_nais _ wfN with "[Hf]") as "#Hinvf".
       by iApply (later_intro with "Hf").
       iMod (na_inv_alloc logrel_nais _ wf0N with "[Hf0]") as "#Hinvf0".
@@ -2688,11 +3793,10 @@ Definition spec4 idf4 i4 l4 f4 isStack :=
       instantiate (1 := ∃ len, N.of_nat m↦[wmlength] len ∗ ⌜  
                                         
       by iApply (later_intro with "Hmemlength"). *)
-      iSplitL "Hexp0 Hexp1 Hexp2 Hexp3 Hexp4".
+      iSplitL "Hexp0 Hexp1 Hexp2 Hexp3 Hexp4 Hexp5 Hexp6".
       unfold import_resources_host.
       iFrame. by iModIntro.
-      iSplitL "Hf Hf0 Hf1 Hf2 Hf3".
-      unfold import_resources_host.
+      iSplitL "Hf Hf0 Hf1 Hf2 Hf3 Hf4 Htab".
       unfold import_resources_wasm_typecheck => /=.
 (*      iMod (na_inv_acc with "Hinvf Hown") as "(Hf & Hown & Hclosef)".
       admit. done.
@@ -2719,27 +3823,42 @@ Definition spec4 idf4 i4 l4 f4 isStack :=
       iSplitL "Hf0".
       iExists _ ; iFrame.
       iPureIntro.
-      rewrite lookup_insert_ne ; last lia.
+      rewrite lookup_insert_ne ; last assumption.
       rewrite lookup_insert.
       split => //.
       iSplitL "Hf1".
       iExists _ ; iFrame.
       iPureIntro.
-      do 2 (rewrite lookup_insert_ne ; last lia).
+      do 2 (rewrite lookup_insert_ne ; last assumption).
       rewrite lookup_insert.
       split => //.
       iSplitL "Hf2".
       iExists _ ; iFrame.
       iPureIntro.
-      do 3 (rewrite lookup_insert_ne ; last lia).
+      do 3 (rewrite lookup_insert_ne ; last assumption).
+      rewrite lookup_insert.
+      split => //.
+      iSplitL "Hf3".
+      iExists _ ; iFrame.
+      iPureIntro.
+      do 4 (rewrite lookup_insert_ne ; last assumption).
+      rewrite lookup_insert.
+      split => //.
+      iSplitL "Hf4".
+      iExists _ ; iFrame.
+      iPureIntro.
+      do 5 (rewrite lookup_insert_ne ; last assumption).
       rewrite lookup_insert.
       split => //.
       iSplitL ; last done.
-      iExists _ ; iFrame.
+      iExists _, _ ; iFrame.
       iPureIntro.
-      do 4 (rewrite lookup_insert_ne ; last lia).
       rewrite lookup_insert.
       split => //.
+      iSplitR.
+      iPureIntro.
+      simpl.
+      lia.
       iSplitL "Hmemlength" ; first done.
     - iSplitR. iIntros "!>" (fr addr Φ) "!> (Hf & Hwf & Hlen & % & % & %) HΦ".
       iApply wp_wand_r.
@@ -2775,7 +3894,7 @@ Definition spec4 idf4 i4 l4 f4 isStack :=
         lia.
         iIntros (w) "H".
         iDestruct "H" as (k) "(-> & H & Hf)" => /=.
-        iDestruct "Hf" as (f4) "[Hf %Hf4]".
+        iDestruct "Hf" as (f5) "[Hf %Hf4]".
         iApply (wp_wand_ctx with "[H Hf Hf0]").
         iApply (wp_val_return with "Hf") => //.
         iIntros "Hf".
@@ -2791,8 +3910,8 @@ Definition spec4 idf4 i4 l4 f4 isStack :=
                            {|
                              inst_types :=
                                [Tf [] [T_i32]; Tf [T_i32] [T_i32]; Tf [T_i32; T_i32] []];
-                             inst_funcs := [f; f0; f1; f2; f3];
-                             inst_tab := [];
+                             inst_funcs := [f; f0; f1; f2; f3;f4];
+                             inst_tab := [t];
                              inst_memory := [m];
                              inst_globs := []
                            |} (Tf [] [T_i32]) [T_i32]
@@ -2824,8 +3943,8 @@ Definition spec4 idf4 i4 l4 f4 isStack :=
                            {|
                              inst_types :=
                                [Tf [] [T_i32]; Tf [T_i32] [T_i32]; Tf [T_i32; T_i32] []];
-                             inst_funcs := [f; f0; f1; f2; f3];
-                             inst_tab := [];
+                             inst_funcs := [f; f0; f1; f2; f3; f4];
+                             inst_tab := [t];
                              inst_memory := [m];
                              inst_globs := []
                            |} (Tf [] [T_i32]) [T_i32]
@@ -2892,10 +4011,10 @@ Definition spec4 idf4 i4 l4 f4 isStack :=
         iFrame.
         repeat iSplit ; iPureIntro => //=.
         lia.
-        lia.
+        by destruct H.
         iIntros (w) "H".
         iDestruct "H" as (k) "(-> & H & %Hk & Hf)" => /=.
-        iDestruct "Hf" as (f4) "[Hf %Hf4]".
+        iDestruct "Hf" as (f5) "[Hf %Hf4]".
         iApply (wp_wand_ctx with "[H Hf Hf0]").
         iApply (wp_val_return with "Hf") => //.
         iIntros "Hf".
@@ -2911,8 +4030,8 @@ Definition spec4 idf4 i4 l4 f4 isStack :=
                               inst_types :=
                                 [Tf [] [T_i32]; Tf [T_i32] [T_i32];
                                 Tf [T_i32; T_i32] []];
-                              inst_funcs := [f; f0; f1; f2; f3];
-                              inst_tab := [];
+                              inst_funcs := [f; f0; f1; f2; f3 ; f4];
+                              inst_tab := [t];
                               inst_memory := [m];
                               inst_globs := []
                             |} (Tf [T_i32] [T_i32]) []
@@ -2939,8 +4058,8 @@ Definition spec4 idf4 i4 l4 f4 isStack :=
                               inst_types :=
                                 [Tf [] [T_i32]; Tf [T_i32] [T_i32];
                                 Tf [T_i32; T_i32] []];
-                              inst_funcs := [f; f0; f1; f2; f3];
-                              inst_tab := [];
+                              inst_funcs := [f; f0; f1; f2; f3; f4];
+                              inst_tab := [t];
                               inst_memory := [m];
                               inst_globs := []
                             |} (Tf [T_i32] [T_i32]) []
@@ -2990,10 +4109,10 @@ Definition spec4 idf4 i4 l4 f4 isStack :=
         iFrame.
         repeat iSplit ; iPureIntro => //=.
         lia.
-        lia.
+        by destruct H.
         iIntros (w) "H".
         iDestruct "H" as (k) "(-> & H & %Hk & Hf)" => /=.
-        iDestruct "Hf" as (f4) "[Hf %Hf4]".
+        iDestruct "Hf" as (f5) "[Hf %Hf4]".
         iApply (wp_wand_ctx with "[H Hf Hf0]").
         iApply (wp_val_return with "Hf") => //.
         iIntros "Hf".
@@ -3009,8 +4128,8 @@ Definition spec4 idf4 i4 l4 f4 isStack :=
                               inst_types :=
                                 [Tf [] [T_i32]; Tf [T_i32] [T_i32];
                                 Tf [T_i32; T_i32] []];
-                              inst_funcs := [f; f0; f1; f2; f3];
-                              inst_tab := [];
+                              inst_funcs := [f; f0; f1; f2; f3 ; f4];
+                              inst_tab := [t];
                               inst_memory := [m];
                               inst_globs := []
                             |} (Tf [T_i32] [T_i32]) []
@@ -3037,8 +4156,8 @@ Definition spec4 idf4 i4 l4 f4 isStack :=
                               inst_types :=
                                 [Tf [] [T_i32]; Tf [T_i32] [T_i32];
                                 Tf [T_i32; T_i32] []];
-                              inst_funcs := [f; f0; f1; f2; f3];
-                              inst_tab := [];
+                              inst_funcs := [f; f0; f1; f2; f3 ; f4];
+                              inst_tab := [t];
                               inst_memory := [m];
                               inst_globs := []
                             |} (Tf [T_i32] [T_i32]) []
@@ -3089,10 +4208,10 @@ Definition spec4 idf4 i4 l4 f4 isStack :=
         repeat iSplit ; iPureIntro => //=.
         lia.
         lia.
-        lia.
+        by destruct H.
         iIntros (w) "H".
         iDestruct "H" as "(-> & Hs & Hf)" => /=.
-        iDestruct "Hf" as (f4) "[Hf %Hf4]".
+        iDestruct "Hf" as (f5) "[Hf %Hf4]".
         iApply (wp_wand_ctx with "[Hs Hf Hf0]").
         iApply (wp_val_return with "Hf") => //.
         iIntros "Hf".
@@ -3101,15 +4220,15 @@ Definition spec4 idf4 i4 l4 f4 isStack :=
         unfold IntoVal.
         apply of_to_val => //.
         iFrame.
-        instantiate (1 := λ v, (⌜ v = immV [a] ⌝ ∗
+        instantiate (1 := λ v, (⌜ v = immV [_] ⌝ ∗
                                            isStack v0 s0 m ∗
                                             N.of_nat f2↦[wf]FC_func_native
                             {|
                               inst_types :=
                                 [Tf [] [T_i32]; Tf [T_i32] [T_i32];
                                 Tf [T_i32; T_i32] []];
-                              inst_funcs := [f; f0; f1; f2; f3];
-                              inst_tab := [];
+                              inst_funcs := [f; f0; f1; f2; f3 ; f4];
+                              inst_tab := [t];
                               inst_memory := [m];
                               inst_globs := []
                             |} (Tf [T_i32] [T_i32]) [T_i32]
@@ -3129,15 +4248,15 @@ Definition spec4 idf4 i4 l4 f4 isStack :=
         iSimpl.         
         iApply (wp_frame_value with "Hf") => //.
         iNext.
-        instantiate (1 := λ v,  (⌜ v = immV [a] ⌝ ∗
+        instantiate (1 := λ v,  (⌜ v = immV [_] ⌝ ∗
                                             isStack v0 s0 m ∗
                                             N.of_nat f2↦[wf]FC_func_native
                                             {|
                               inst_types :=
                                 [Tf [] [T_i32]; Tf [T_i32] [T_i32];
                                 Tf [T_i32; T_i32] []];
-                              inst_funcs := [f; f0; f1; f2; f3];
-                              inst_tab := [];
+                              inst_funcs := [f; f0; f1; f2; f3 ; f4];
+                              inst_tab := [t];
                               inst_memory := [m];
                               inst_globs := []
                             |} (Tf [T_i32] [T_i32]) [T_i32]
@@ -3153,7 +4272,7 @@ Definition spec4 idf4 i4 l4 f4 isStack :=
       iIntros (w) "[(-> & Hs & Hf0) Hf]".
       iApply "HΦ".
       by iFrame.
-    - iIntros "!>" (a v0 s0 vs Φ) "!> (Hf & Hf0 & %H & %Ha & %Hlen & Hs) HΦ".
+    - iSplitR. iIntros "!>" (a v0 s0 vs Φ) "!> (Hf & Hf0 & %H & %Ha & %Hlen & Hs) HΦ".
       iApply wp_wand_r.
       iSplitR "HΦ".
       { rewrite (separate2 _ (i32const _) _).
@@ -3184,9 +4303,9 @@ Definition spec4 idf4 i4 l4 f4 isStack :=
         repeat iSplit ; iPureIntro => //=.
         lia.
         lia.
-        lia.
+        by destruct H.
         iIntros (w) "(-> & Hs & Hf)".
-        iDestruct "Hf" as (f4) "[Hf %Hf4]".
+        iDestruct "Hf" as (f5) "[Hf %Hf4]".
         iApply (wp_wand_ctx with "[Hs Hf Hf0]").
         iApply (wp_val_return with "Hf") => //.
         iIntros "Hf".
@@ -3202,8 +4321,8 @@ Definition spec4 idf4 i4 l4 f4 isStack :=
                               inst_types :=
                                 [Tf [] [T_i32]; Tf [T_i32] [T_i32];
                                 Tf [T_i32; T_i32] []];
-                              inst_funcs := [f; f0; f1; f2; f3];
-                              inst_tab := [];
+                              inst_funcs := [f; f0; f1; f2; f3;f4];
+                              inst_tab := [t];
                               inst_memory := [m];
                               inst_globs := []
                             |} (Tf [T_i32; T_i32] []) [T_i32]
@@ -3231,8 +4350,8 @@ Definition spec4 idf4 i4 l4 f4 isStack :=
                               inst_types :=
                                 [Tf [] [T_i32]; Tf [T_i32] [T_i32];
                                 Tf [T_i32; T_i32] []];
-                              inst_funcs := [f; f0; f1; f2; f3];
-                              inst_tab := [];
+                              inst_funcs := [f; f0; f1; f2; f3 ; f4];
+                              inst_tab := [t];
                               inst_memory := [m];
                               inst_globs := []
                             |} (Tf [T_i32; T_i32] []) [T_i32]
@@ -3250,49 +4369,170 @@ Definition spec4 idf4 i4 l4 f4 isStack :=
       iIntros (w) "[(-> & Hs & Hf0) Hf]".
       iApply "HΦ".
       by iFrame.
+    - iIntros "!>" (f5 fi v0 s0 a cl Φ Ψ Ξ)
+              "!> (Hf & Hf0 & % & %Hs & Hs & HΦ & Htab & Hcl & %Hclt & #Hspec) HΞ".
+      iApply wp_wand_r.
+      iSplitR "HΞ".
+      { rewrite (separate2 _ (i32const _) _).
+        rewrite - (app_nil_r [AI_basic _]).
+        (* iApply wp_wasm_empty_ctx.
+        iApply wp_base_push => //.
+        iApply (wp_call_ctx with "Hf") => //=.
+        iIntros "!> Hf".
+        iApply wp_base_pull.
+        rewrite app_nil_r.
+        iApply wp_wasm_empty_ctx. *)
+        iApply (wp_invoke_native with "Hf Hf0") => //.
+        iIntros "!> [Hf Hf0]".
+        iSimpl.
+        iApply (wp_frame_bind with "Hf").
+        iIntros "Hf".
+        rewrite - (app_nil_l [AI_basic (BI_block _ _)]).
+        iApply (wp_block with "Hf") => //.
+        iIntros "!> Hf".
+        iApply (wp_label_bind with "[Hs Hf Hf0 HΦ Htab Hcl]") ; last first.
+        iPureIntro.
+        unfold lfilled, lfill => /=.
+        instantiate (5 := []) => /=.
+        rewrite app_nil_r.
+        done.
+        iApply (spec_stack_map with "[Hs Hf HΦ Hcl Htab]").        
+        iFrame.
+        repeat iSplit ; try iPureIntro => //=.
+        lia.
+ (*       iIntros (u fc) "!>". iIntros (Φ0) "(Hu & % & H)".
+        iApply "Hspec".
+        iFrame. *)
+        iExact "Hspec".
+        iIntros (w) "(-> & Hs & Hf)".
+        iDestruct "Hf" as (f6) "[Hf %Hf4]".
+        iApply (wp_wand_ctx with "[Hs Hf Hf0]").
+        iApply (wp_val_return with "Hf") => //.
+        iIntros "Hf".
+        iSimpl.
+        iApply wp_value => //=.
+        unfold IntoVal.
+        apply of_to_val => //.
+        iFrame.
+        instantiate (1 := λ v, (⌜ v = immV [] ⌝ ∗
+                                           ( ∃ s', isStack v0 s' m ∗ stackAll2 s0 s' Ψ) ∗
+                                           N.of_nat f4↦[wf]FC_func_native
+                            {|
+                              inst_types :=
+                                [Tf [] [T_i32]; Tf [T_i32] [T_i32];
+                                Tf [T_i32; T_i32] []];
+                              inst_funcs := [f; f0; f1; f2; f3;f4];
+                              inst_tab := [t];
+                              inst_memory := [m];
+                              inst_globs := []
+                            |} (Tf [T_i32; T_i32] []) [T_i32 ; T_i32 ]
+                           [BI_get_local 1; BI_load T_i32 None N.zero N.zero;
+                            BI_set_local 3; BI_get_local 1;
+                            BI_const (VAL_int32 (Wasm_int.Int32.repr 4));
+                            BI_binop T_i32 (Binop_i BOI_add); 
+                            BI_set_local 2;
+                            BI_block (Tf [] [])
+                              [BI_loop (Tf [] [])
+                                 [BI_get_local 2; BI_get_local 3;
+                                 BI_relop T_i32 (Relop_i (ROI_ge SX_U)); 
+                                 BI_br_if 1; BI_get_local 2; 
+                                 BI_get_local 2; BI_get_local 2;
+                                 BI_load T_i32 None N.zero N.zero; 
+                                 BI_get_local 0; BI_call_indirect 1;
+                                 BI_store T_i32 None N.zero N.zero; 
+                                 bi32const 4; BI_binop T_i32 (Binop_i BOI_add);
+                                 BI_set_local 2; BI_br 0]]])%I).
+        iSimpl.
+        iFrame.
+        done.
+        iIntros (w) "[(-> & H &  Hf0) Hf]".
+        iExists _.
+        iFrame.
+        iIntros "Hf".
+        iSimpl.         
+        iApply (wp_frame_value with "Hf") => //.
+        iNext.
+         instantiate (1 := λ v, (⌜ v = immV [] ⌝ ∗
+                                            ( ∃ s', isStack v0 s' m ∗ stackAll2 s0 s' Ψ) ∗
+                                 N.of_nat f4↦[wf]FC_func_native
+                            {|
+                              inst_types :=
+                                [Tf [] [T_i32]; Tf [T_i32] [T_i32];
+                                Tf [T_i32; T_i32] []];
+                              inst_funcs := [f; f0; f1; f2; f3; f4];
+                              inst_tab := [t];
+                              inst_memory := [m];
+                              inst_globs := []
+                            |} (Tf [T_i32; T_i32] []) [T_i32; T_i32]
+                            [BI_get_local 1; BI_load T_i32 None N.zero N.zero;
+                            BI_set_local 3; BI_get_local 1;
+                            BI_const (VAL_int32 (Wasm_int.Int32.repr 4));
+                            BI_binop T_i32 (Binop_i BOI_add); 
+                            BI_set_local 2;
+                            BI_block (Tf [] [])
+                              [BI_loop (Tf [] [])
+                                 [BI_get_local 2; BI_get_local 3;
+                                 BI_relop T_i32 (Relop_i (ROI_ge SX_U)); 
+                                 BI_br_if 1; BI_get_local 2; 
+                                 BI_get_local 2; BI_get_local 2;
+                                 BI_load T_i32 None N.zero N.zero; 
+                                 BI_get_local 0; BI_call_indirect 1;
+                                 BI_store T_i32 None N.zero N.zero; 
+                                 bi32const 4; BI_binop T_i32 (Binop_i BOI_add);
+                                 BI_set_local 2; BI_br 0]]])%I).
+        iSimpl.
+        iFrame.
+        iFrame.
+        done. }
+      iIntros (w) "[(-> & Hs & Hf0) Hf]".
+      iApply "HΞ".
+      by iFrame.
   Qed. 
 
   
 
-  Lemma instantiate_stack_client_spec (s: stuckness) E hv0 hv1 hv2 hv3 hv4 hv5 :
+  Lemma instantiate_stack_client_spec (s: stuckness) E hv0 hv1 hv2 hv3 hv4 hv5 hv6 hv7 :
     0%N ↪[mods] stack_module -∗
      1%N ↪[mods] client_module -∗
-     ( [∗ list] k↦hvk ∈ [hv0 ; hv1 ; hv2 ; hv3 ; hv4 ; hv5], N.of_nat k↪[vis] hvk) -∗
+     ( [∗ list] k↦hvk ∈ [hv0 ; hv1 ; hv2 ; hv3 ; hv4 ; hv5 ; hv6 ; hv7], N.of_nat k↪[vis] hvk) -∗
      WP ((stack_instantiate , []) : host_expr)
      @ s; E
             {{ v,
                 0%N ↪[mods] stack_module ∗
                  1%N ↪[mods] client_module ∗
                  ∃ idg name,
-                   5%N ↪[vis] {| modexp_name := name ;
+                   7%N ↪[vis] {| modexp_name := name ;
                                 modexp_desc := MED_global (Mk_globalidx idg) |} ∗
-                    (N.of_nat idg ↦[wg] {| g_mut := MUT_mut ; g_val := value_of_int 2%Z |} ∨
+                    (N.of_nat idg ↦[wg] {| g_mut := MUT_mut ; g_val := value_of_int 20%Z |} ∨
                        N.of_nat idg ↦[wg] {| g_mut := MUT_mut ; g_val := value_of_int (-1)%Z |}) }}.
   Proof.
-    iIntros "Hmod0 Hmod1 (Hvis0 & Hvis1 & Hvis2 & Hvis3 & Hvis4 & Hvis5 & _)".
-    iApply (wp_seq_host_nostart with "[$Hmod0] [Hvis0 Hvis1 Hvis2 Hvis3 Hvis4]") => //.
+    iIntros "Hmod0 Hmod1 (Hvis0 & Hvis1 & Hvis2 & Hvis3 & Hvis4 & Hvis5 & Hvis6 & Hvis7 &  _)".
+    iApply (wp_seq_host_nostart
+             with "[$Hmod0] [Hvis0 Hvis1 Hvis2 Hvis3 Hvis4 Hvis5 Hvis6]") => //.
     - iIntros "Hmod0".
-      iApply weakestpre.wp_mono ; last iApply (instantiate_stack_spec with "Hmod0 [Hvis0 Hvis1 Hvis2 Hvis3 Hvis4]").
+      iApply weakestpre.wp_mono ;
+        last iApply (instantiate_stack_spec
+                      with "Hmod0 [Hvis0 Hvis1 Hvis2 Hvis3 Hvis4 Hvis5 Hvis6]").
       2:{ iSplitL "Hvis0" ; first done.
           iSplitL "Hvis1" ; first done.
           iSplitL "Hvis2" ; first done.
           iSplitL "Hvis3" ; first done.
+          iSplitL "Hvis4" ; first done.
+          iSplitL "Hvis5" ; first done.
           by iSplitL. }
       iIntros (v) "[? H]".
       iFrame.
       by iApply "H".
     - iIntros (w) "Hes1 Hmod0".
-      iDestruct "Hes1" as (idf0 idf1 idf2 idf3 idf4 name0 name1 name2 name3 name4) "Hes1".
-      iDestruct "Hes1" as (f0 f1 f2 f3 f4 i0 i1 i2 i3 i4) "Hes1".  
-      iDestruct "Hes1" as (l0 l1 l2 l3 l4) "Hes1".
-      iDestruct "Hes1" as (isStack nextStackAddrIs)
-                            "(Himport & Himp_type & Hnextaddr & #Hspec0 & #Hspec1 & #Hspec2 & #Hspec3 & #Hspec4)".
-(*      "(Hvis0 & Hvis1 & Hvis2 & Hvis3 & Hvis4 & Hlen & Hwf0 & Hwf1 & Hwf2 & Hwf3 & Hwf4 &
-      #Hspec0 & #Hspec1 & #Hspec2 & #Hspec3 & #Hspec4)". *)
+      iDestruct "Hes1" as (idf0 idf1 idf2 idf3 idf4 idf5 idt) "Hes1".
+      iDestruct "Hes1" as (name0 name1 name2 name3 name4 name5 name6) "Hes1".
+      iDestruct "Hes1" as (f0 f1 f2 f3 f4 f5) "Hes1".
+      iDestruct "Hes1" as (i0 i1 i2 i3 i4 i5) "Hes1".  
+      iDestruct "Hes1" as (l0 l1 l2 l3 l4 l5) "Hes1".
+      iDestruct "Hes1" as (tab isStack nextStackAddrIs)
+                            "(Himport & Himp_type & %Htab & Hnextaddr & #Hspec0 & #Hspec1 & #Hspec2 & #Hspec3 & #Hspec4 & #Hspec5)".
       iFrame "Hmod0".
-(*      iApply (weakestpre.wp_strong_mono s _ E with "[Hmod1 Hvis0 Hvis1 Hvis2 Hvis3 Hvis4 Hvis5 Hwf0 Hwf1 Hwf2 Hwf3 Hwf4 Hlen]") ; try done. *)
-
-      iApply (instantiation_spec_operational_start with "[Hmod1 Himport Himp_type Hvis5]") ; try exact module_typing_client.
+      iApply (instantiation_spec_operational_start with "[Hmod1 Himport Himp_type Hvis7]") ; try exact module_typing_client.
     - by unfold client_module.
     - unfold instantiation_resources_pre.
       iFrame.
@@ -3360,12 +4600,21 @@ Definition spec4 idf4 i4 l4 f4 isStack :=
       split => //. *)
       
     - unfold export_ownership_host => /=.
-      iSplit; last done.
-      by iExists _. 
+      repeat iSplit.
+      by iExists _.
+      done.
+      done.
+      iPureIntro ; unfold module_elem_bound_check_gmap ; simpl.
+      apply Forall_cons.
+      split ; last done.
+      simpl.
+      rewrite lookup_insert.
+      done.
+      iPureIntro ; unfold module_data_bound_check_gmap ; simpl ; done.
     - iIntros (idnstart) "Hf Hres".
       unfold instantiation_resources_post.
       iDestruct "Hres" as "(Hmod1 & Himphost & Himpwasm & Hinst)".
-      iDestruct "Hinst" as (inst g_inits) "(%Hinst & Hexpwasm & Hexphost)".
+      iDestruct "Hinst" as (inst g_inits t_inits m_inits) "(%Hinst & %Hival & Hexpwasm & Hexphost)".
       destruct Hinst as (Hinsttype & Hinstfunc & Hinsttab & Hinstmem & Hinstglob & Hstart).
       unfold module_inst_resources_wasm, module_export_resources_host => /=.
       destruct inst => /=.
@@ -3373,16 +4622,19 @@ Definition spec4 idf4 i4 l4 f4 isStack :=
       unfold module_inst_resources_func, module_inst_resources_tab,
         module_inst_resources_mem, module_inst_resources_glob => /=.
       unfold big_sepL2 => /=.
-      do 5 (destruct inst_funcs as [| ? inst_funcs] ; first by iExFalso ; iExact "Hexpwf").
-      rewrite drop_0.
-      destruct inst_funcs ; first by iExFalso ; iExact "Hexpwf".
+      do 7 (destruct inst_funcs as [| ? inst_funcs] ; first by iExFalso ; iExact "Hexpwf").
+      simpl.
       iDestruct "Hexpwf" as "[Hwfcl Hexpwf]".
+      destruct inst_funcs ; first by iExFalso ; iExact "Hexpwf".
+      iDestruct "Hexpwf" as "[Hwfsq Hexpwf]".
       destruct inst_funcs ; last by iExFalso ; iExact "Hexpwf".
-      destruct inst_tab ; last by iExFalso ; iExact "Hexpwt".
+(*      destruct inst_tab ; first by iExFalso ; iExact "Hexpwt".
+      iDestruct "Hexpwt" as "[Hwt Hexpwt]".
+      destruct inst_tab ; last by iExFalso ; iExact "Hexpwt". *)
       destruct inst_memory ; last by iExFalso ; iExact "Hexpwm".
       destruct inst_globs as [| g inst_globs] ; first by iExFalso ; iExact "Hexpwg". 
       iDestruct "Hexpwg" as "[Hwg Hexpwg]".
-      destruct (nth_error g_inits g) eqn:Hg ; try by iExFalso ; iExact "Hwg".
+      destruct g_inits eqn:Hg ; try by iExFalso ; iExact "Hwg".
       destruct inst_globs ; last by iExFalso ; iExact "Hexpwg". 
       iDestruct "Hexphost" as "[Hexphost _]".
       iDestruct "Hexphost" as (name) "Hexphost" => /=.
@@ -3393,40 +4645,55 @@ Definition spec4 idf4 i4 l4 f4 isStack :=
       destruct name0 ; first done ; iDestruct "Himpwasm" as "[Himpw2 Himpwasm]".
       destruct name0 ; first done ; iDestruct "Himpwasm" as "[Himpw3 Himpwasm]".
       destruct name0 ; first done ; iDestruct "Himpwasm" as "[Himpw4 _]". *) 
-      iDestruct "Himpwasm" as "(%Hdom & Himpw0 & Himpw1 & Himpw2 & Himpw3 & Himpw4 & _)". 
+      iDestruct "Himpwasm" as "(%Hdom & Himpw0 & Himpw1 & Himpw2 & Himpw3 & Himpw4 & Himpw5 & Htab & _)". 
       iDestruct "Himpw0" as (cl0) "[Himpfcl0 %Hcltype0]".
       iDestruct "Himpw1" as (cl1) "[Himpfcl1 %Hcltype1]".
       iDestruct "Himpw2" as (cl2) "[Himpfcl2 %Hcltype2]".
       iDestruct "Himpw3" as (cl3) "[Himpfcl3 %Hcltype3]".
       iDestruct "Himpw4" as (cl4) "[Himpfcl4 %Hcltype4]".
+      iDestruct "Himpw5" as (cl5) "[Himpfcl5 %Hcltype5]".
+      iDestruct "Htab" as (tab0 tt) "[Htab %Htab0]".
       iDestruct (mapsto_frac_ne with "Himpfcl0 Himpfcl1") as "%H01" ; first by eauto.
       iDestruct (mapsto_frac_ne with "Himpfcl0 Himpfcl2") as "%H02" ; first by eauto.
       iDestruct (mapsto_frac_ne with "Himpfcl0 Himpfcl3") as "%H03" ; first by eauto.
       iDestruct (mapsto_frac_ne with "Himpfcl0 Himpfcl4") as "%H04" ; first by eauto.
+      iDestruct (mapsto_frac_ne with "Himpfcl0 Himpfcl5") as "%H05" ; first by eauto.
       iDestruct (mapsto_frac_ne with "Himpfcl1 Himpfcl2") as "%H12" ; first by eauto.
       iDestruct (mapsto_frac_ne with "Himpfcl1 Himpfcl3") as "%H13" ; first by eauto.
       iDestruct (mapsto_frac_ne with "Himpfcl1 Himpfcl4") as "%H14" ; first by eauto.
+      iDestruct (mapsto_frac_ne with "Himpfcl1 Himpfcl5") as "%H15" ; first by eauto.
       iDestruct (mapsto_frac_ne with "Himpfcl2 Himpfcl3") as "%H23" ; first by eauto.
       iDestruct (mapsto_frac_ne with "Himpfcl2 Himpfcl4") as "%H24" ; first by eauto.
+      iDestruct (mapsto_frac_ne with "Himpfcl2 Himpfcl5") as "%H25" ; first by eauto.
       iDestruct (mapsto_frac_ne with "Himpfcl3 Himpfcl4") as "%H34" ; first by eauto.
+      iDestruct (mapsto_frac_ne with "Himpfcl3 Himpfcl5") as "%H35" ; first by eauto.
+      iDestruct (mapsto_frac_ne with "Himpfcl4 Himpfcl5") as "%H45" ; first by eauto.
+(*      assert (forall a b, N.of_nat a <> N.of_nat b -> a <> b) as Hneq.
+      { intros ; intro. by subst. }
+      apply Hneq in H01, H02, H03, H04, H05, H12, H13, H14, H15, H23, H24, H25, H34, H35, H45. *)
       rewrite lookup_insert in Hcltype0.
       destruct Hcltype0 as [Hcl _] ; inversion Hcl ; subst ; clear Hcl.
-      rewrite lookup_insert_ne in Hcltype1 ; last lia.
+      rewrite lookup_insert_ne in Hcltype1 ; last assumption.
       rewrite lookup_insert in Hcltype1.
       destruct Hcltype1 as [Hcl _] ; inversion Hcl ; subst ; clear Hcl.
-      do 2 (rewrite lookup_insert_ne in Hcltype2 ; last lia).
+      do 2 (rewrite lookup_insert_ne in Hcltype2 ; last assumption).
       rewrite lookup_insert in Hcltype2.
       destruct Hcltype2 as [Hcl _] ; inversion Hcl ; subst ; clear Hcl.
-      do 3 (rewrite lookup_insert_ne in Hcltype3 ; last lia).
+      do 3 (rewrite lookup_insert_ne in Hcltype3 ; last assumption).
       rewrite lookup_insert in Hcltype3.
       destruct Hcltype3 as [Hcl _] ; inversion Hcl ; subst ; clear Hcl.
-      do 4 (rewrite lookup_insert_ne in Hcltype4 ; last lia).
+      do 4 (rewrite lookup_insert_ne in Hcltype4 ; last assumption).
       rewrite lookup_insert in Hcltype4.
-      destruct Hcltype4 as [Hcl _] ; inversion Hcl ; subst ; clear Hcl. 
+      destruct Hcltype4 as [Hcl _] ; inversion Hcl ; subst ; clear Hcl.
+      do 5 (rewrite lookup_insert_ne in Hcltype5 ; last assumption).
+      rewrite lookup_insert in Hcltype5.
+      destruct Hcltype5 as [Hcl _] ; inversion Hcl ; subst ; clear Hcl.
+      rewrite lookup_insert in Htab0.
+      destruct Htab0 as [Htab0 _] ; inversion Htab0 ; subst ; clear Htab0.
       simpl in * ; subst. 
       unfold ext_func_addrs in Hinstfunc ; simpl in Hinstfunc.
       unfold prefix in Hinstfunc.
-      destruct Hinstfunc as [l Hinstfunc].
+      destruct Hinstfunc as [ll Hinstfunc].
       inversion Hinstfunc ; subst ; clear Hinstfunc.
       unfold check_start in Hstart.
       simpl in Hstart.
@@ -3447,7 +4714,7 @@ Definition spec4 idf4 i4 l4 f4 isStack :=
       done. done. done. done.
       iIntros "!> Hf".
       iApply (wp_label_bind with
-               "[Hwg Hf Himpfcl0 Himpfcl1 Himpfcl2 Himpfcl3 Himpfcl4 Hexphost Hnextaddr]") ; last first.
+               "[Hwg Htab Hwfsq Hf Himpfcl0 Himpfcl1 Himpfcl2 Himpfcl3 Himpfcl4 Himpfcl5 Hexphost Hnextaddr]") ; last first.
       iPureIntro.
       unfold lfilled, lfill => /=.
       instantiate (5 := []) => /=.
@@ -3495,20 +4762,7 @@ Definition spec4 idf4 i4 l4 f4 isStack :=
         iSimpl.
         iSimpl in "Hf".
         instantiate (1 := λ v, (⌜ v = immV [VAL_int32 (Wasm_int.Int32.repr k)] ⌝
-                                           ∗ ↪[frame] {|
-                                             f_locs := [VAL_int32 (Wasm_int.Int32.repr k)];
-                                             f_inst :=
-                                             {|
-                                               inst_types :=
-                                               [Tf [] []; Tf [] [T_i32]; Tf [T_i32] [T_i32];
-                                                Tf [T_i32; T_i32] []];
-                                               inst_funcs := [idf0; idf1; idf2; idf3; idf4; idnstart];
-                                               inst_tab := [];
-                                               inst_memory := [];
-                                               inst_globs := [g]
-                                             |}
-                                           |}
-                               )%I).
+                                           ∗ ↪[frame] _)%I). 
         by iFrame.
         by iIntros "!> [%H _]".
         iIntros (w0) "[-> Hf]".
@@ -3540,19 +4794,7 @@ Definition spec4 idf4 i4 l4 f4 isStack :=
                                               N.of_nat g↦[wg] {| g_mut := MUT_mut ; g_val := v |} ∨
                                     ⌜ exists sh, v1 = retV sh ⌝ ∗
                                                       N.of_nat g↦[wg] {| g_mut := MUT_mut ; g_val := value_of_int (-1)%Z |}) ∗
-                                                                                                                             ↪[frame] {|
-                                                                                                                               f_locs := [VAL_int32 (Wasm_int.Int32.repr k)];
-                                                                                                                               f_inst :=
-                                                                                                                               {|
-                                                                                                                                 inst_types :=
-                                                                                                                                 [Tf [] []; Tf [] [T_i32]; Tf [T_i32] [T_i32];
-                                                                                                                                  Tf [T_i32; T_i32] []];
-                                                                                                                                 inst_funcs := [idf0; idf1; idf2; idf3; idf4; idnstart];
-                                                                                                                                 inst_tab := [];
-                                                                                                                                 inst_memory := [];
-                                                                                                                                 inst_globs := [g]                                                                                                                                                                                                                              |}
-                                                                                                                             |} )%I).
-        
+                                                                                                                             ↪[frame] _)%I ).         
         destruct ( decide ( k = (* Wasm_int.Int32.modulus *) - 1)%Z ).
         + { subst. iSimpl.
             iApply (wp_if_true with "Hf") => //.
@@ -3651,20 +4893,8 @@ Definition spec4 idf4 i4 l4 f4 isStack :=
             iIntros (w0) "[-> Hf]".
             iSimpl.
             instantiate (1 := λ v, (⌜ v = immV [value_of_int 4%Z ; value_of_int k] ⌝ ∗
-                                               ↪[frame] {|
-                                                 f_locs := [VAL_int32 (Wasm_int.Int32.repr k)];
-                                                 f_inst :=
-                                                 {|
-                                                   inst_types :=
-                                                   [Tf [] []; Tf [] [T_i32]; Tf [T_i32] [T_i32];
-                                                    Tf [T_i32; T_i32] []];
-                                                   inst_funcs := [idf0; idf1; idf2; idf3; idf4; idnstart];
-                                                   inst_tab := [];
-                                                   inst_memory := [];
-                                                   inst_globs := [g]
-                                               |}
-                                             |})%I).
-          by iFrame.
+                                               ↪[frame] _)%I ). 
+            by iFrame.
           by iIntros "!> [%H _]".
           iIntros (w0) "[-> Hf]".
           iSimpl.
@@ -3693,7 +4923,7 @@ Definition spec4 idf4 i4 l4 f4 isStack :=
           iIntros (w0) "(-> & Hs & Himpfcl4 & Hf)".
           iFrame.
           instantiate (1 := λ v, (⌜ v = immV [] ⌝ ∗
-                                             isStack k [VAL_int32 (Wasm_int.int_of_Z i32m 4)] ∗
+                                             isStack k [ (Wasm_int.int_of_Z i32m 4)] ∗
                                              N.of_nat idf4↦[wf]FC_func_native i4 (Tf [T_i32 ; T_i32] []) l4 f4)%I).
           by iFrame.
           iIntros (w0) "[(-> & Hs & Himpfcl4) Hf]".
@@ -3714,20 +4944,8 @@ Definition spec4 idf4 i4 l4 f4 isStack :=
           done.
           iIntros (v0) "[-> Hf]".
           iSimpl.
-          instantiate (1 := λ v, (⌜ v = immV [value_of_int 6 ; value_of_int k] ⌝ ∗
-                                             ↪[frame] {|
-                                               f_locs := [VAL_int32 (Wasm_int.Int32.repr k)];
-                                               f_inst :=
-                                               {|
-                                                 inst_types :=
-                                                 [Tf [] []; Tf [] [T_i32]; Tf [T_i32] [T_i32];
-                                                  Tf [T_i32; T_i32] []];
-                                                 inst_funcs := [idf0; idf1; idf2; idf3; idf4; idnstart];
-                                                 inst_tab := [];
-                                                 inst_memory := [];
-                                                 inst_globs := [g]
-                                               |}
-                                             |})%I).
+          instantiate (1 := λ v, (⌜ v = immV _ ⌝ ∗
+                                             ↪[frame] _)%I).  
           by iFrame.
           by iIntros "!> [%H _]".
           iIntros (w0) "[-> Hf]".
@@ -3757,10 +4975,142 @@ Definition spec4 idf4 i4 l4 f4 isStack :=
           iIntros (w0) "(-> & Hs & Himpfcl4 & Hf)".
           iFrame.
           instantiate (1 := λ v, (⌜ v = immV [] ⌝ ∗
-                                             isStack k [VAL_int32 (Wasm_int.int_of_Z i32m 6) ; value_of_int 4] ∗
+                                             isStack k [_;_] ∗
                                              N.of_nat idf4↦[wf]FC_func_native i4 (Tf [T_i32 ; T_i32] []) l4 f4)%I).
           by iFrame.
           iIntros (w0) "[(-> & Hs & Himpfcl4) Hf]".
+          iSimpl.
+          rewrite (separate2 (AI_basic _)).
+          iApply wp_seq.
+          iSplitR ; last first.
+          iSplitL "Hf".
+          rewrite (separate1 (AI_basic _)).
+          iApply wp_val_app ; first done.
+          iSplitR ; last first.
+          iApply wp_wand_r ; iSplitL.
+          iApply (wp_get_local with "Hf").
+          done.
+          by instantiate (1 := λ v, v = immV _).
+          iIntros (v0) "[-> Hf]".
+          by instantiate (1 := λ v, (⌜ v = immV _ ⌝ ∗ ↪[frame] _)%I) ; iFrame.
+          by iIntros "!> [% _]".
+          iIntros (v0) "[-> Hf]".
+          iSimpl.
+          rewrite (separate3 (i32const 0)).
+          iApply wp_seq.
+          iSplitR ; last first.
+          iSplitL "Hf Himpfcl5 Hs Htab Hwfsq".
+          rewrite (separate2 (i32const _)).
+          rewrite - (app_nil_r [AI_basic (BI_call 5)]).
+          iApply wp_wasm_empty_ctx.
+          iApply wp_base_push => //.
+          iApply (wp_call_ctx with "Hf") => //=.
+          iIntros "!> Hf".
+          iApply wp_base_pull.
+          rewrite app_nil_r.
+          iApply wp_wasm_empty_ctx.
+          iApply ("Hspec5" with "[Hf Himpfcl5 Hs Htab Hwfsq]").
+          iFrame.
+          iSimpl.
+          repeat iSplit ; try iPureIntro.
+          by destruct Hk2.
+          unfold Wasm_int.Int32.max_unsigned, Wasm_int.Int32.modulus.
+          unfold Wasm_int.Int32.wordsize, Integers.Wordsize_32.wordsize.
+          replace (two_power_nat 32) with two32 ; last done.
+          by destruct Hk2 ; lia.
+          instantiate (2 := λ x, True%I).
+          iSplit ; first done.
+          iSplitL "Htab".
+          admit.
+          iSplit ; first done.
+          instantiate (1 := λ x y, ⌜ y = Wasm_int.Int32.imul x x ⌝%I ).
+          iIntros (u fc) "!>". iIntros (Λ) "(_ & -> & Hf & Htab & Hcl) HΛ".
+          rewrite (separate1 _ [AI_invoke _]).
+          iApply wp_wand_r.
+          iSplitL "Hf Hcl".
+          iApply (wp_invoke_native with "Hf Hcl").
+          done.
+          done.
+          done.
+          iIntros "!> [Hf Hcl]".
+          iApply (wp_frame_bind with "Hf").
+          iIntros "Hf".
+          rewrite - (app_nil_l [AI_basic (BI_block _ _)]).
+          iApply (wp_block with "Hf").
+          done.
+          done.
+          done.
+          done.
+          iIntros "!> Hf".
+          iApply (wp_label_bind with "[Hf Hcl]") ; last first.
+          iPureIntro.
+          unfold lfilled, lfill.
+          instantiate (4 := []) => /=.
+          by rewrite app_nil_r.
+          rewrite (separate1 (AI_basic _)).
+          iApply wp_seq.
+          iSplitR ; last first.
+          iSplitL "Hf".
+          iApply (wp_get_local with "Hf").
+          done.
+          by instantiate (1 := λ x, x = immV _).
+          iIntros (w0) "[-> Hf]".
+          iSimpl.
+          rewrite (separate2 (AI_basic _)).
+          iApply wp_seq.
+          iSplitR ; last first.
+          iSplitL "Hf".
+          rewrite (separate1 (AI_basic _)).
+          iApply wp_val_app ; first done.
+          iSplitR ; last first.
+          iApply wp_wand_r.
+          iSplitL.
+          iApply (wp_get_local with "Hf").
+          done.
+          by instantiate (1 := λ x, x = immV _).
+          iIntros (v0) "[-> Hf]".
+          by instantiate (1 := λ x, (⌜ x = immV _ ⌝ ∗ ↪[frame] _)%I) ; iFrame.
+          by iIntros "!> [% _]".
+          iIntros (w0) "[-> Hf]".
+          iSimpl.
+          iApply wp_wand_r.
+          iSplitL "Hf".
+          iApply (wp_binop with "Hf").
+          done.
+          by instantiate (1 := λ x, ⌜ x = immV _ ⌝%I).
+          iIntros (v0) "[-> Hf]".
+          iSimpl.
+          iIntros (lh) "%Hlh".
+          unfold lfilled, lfill in Hlh ; simpl in Hlh.
+          apply b2p in Hlh as ->.
+          iApply wp_wand_r.
+          iSplitL "Hf".
+          iApply (wp_label_value with "Hf") ; first done.
+          by instantiate (1 := λ x, ⌜ x = immV _ ⌝%I).
+          iIntros (v0) "[-> Hf]".
+          iExists _.
+          iFrame.
+          iIntros "Hf".
+          iSimpl.
+          iApply (wp_frame_value with "Hf") ; first done.
+          done.
+          iNext.
+          by instantiate (1 := λ x, (⌜ x = immV _⌝ ∗ N.of_nat f12 ↦[wf] _)%I) ; iFrame.
+          all : try by iIntros "[% _]".
+          iIntros (v0) "[[-> Hcl] Hf]".
+          iApply "HΛ".
+          iFrame.
+          by iExists _.
+          iIntros (w0) "(-> & H & Hwimpcl5 & Hf)".
+          iDestruct "H" as (s') "[Hs Hs']".
+          destruct s' ; first by iExFalso ; iExact "Hs'".
+          iDestruct "Hs'" as "[-> Hs']".
+          destruct s' ; first by iExFalso ; iExact "Hs'".
+          iDestruct "Hs'" as "[-> Hs']".
+          destruct s' ; last by iExFalso ; iExact "Hs'".
+          iFrame.
+          by instantiate (1 := λ x, (⌜ x = immV _ ⌝ ∗ isStack _ _ ∗ N.of_nat idf5 ↦[wf] _)%I) ; iFrame.
+          iIntros (w0) "[(-> & Hs & Himpfcl5) Hf]".
           iSimpl.
           rewrite (separate1 (AI_basic _)).
           iApply wp_seq.
@@ -3796,8 +5146,8 @@ Definition spec4 idf4 i4 l4 f4 isStack :=
           by destruct Hk2 ; lia.
           iIntros (w0) "(-> & Hs & Himpfcl3 & Hf)".
           iFrame.
-          instantiate (1 := λ v, (⌜ v = immV [value_of_int 6] ⌝ ∗
-                                             isStack k [value_of_int 4] ∗
+          instantiate (1 := λ v, (⌜ v = immV _ ⌝ ∗
+                                             isStack k _ ∗
                                              N.of_nat idf3 ↦[wf] FC_func_native i3 (Tf [T_i32] [T_i32]) l3 f3)%I).
           by iFrame.
           iIntros (w0) "[(-> & Hs & Himpfcl3) Hf]".
@@ -3818,20 +5168,8 @@ Definition spec4 idf4 i4 l4 f4 isStack :=
           done.
           iIntros (v0) "[-> Hf]".
           iSimpl.
-          instantiate (1 := λ v, (⌜ v = immV [value_of_int 6 ; value_of_int k] ⌝ ∗
-                                             ↪[frame] {|
-                                               f_locs := [VAL_int32 (Wasm_int.Int32.repr k)];
-                                               f_inst :=
-                                               {|
-                                                 inst_types :=
-                                                 [Tf [] []; Tf [] [T_i32]; Tf [T_i32] [T_i32];
-                                                  Tf [T_i32; T_i32] []];
-                                                 inst_funcs := [idf0; idf1; idf2; idf3; idf4; idnstart];
-                                                 inst_tab := [];
-                                                 inst_memory := [];
-                                                 inst_globs := [g]
-                                               |}
-                                             |})%I).
+          instantiate (1 := λ v, (⌜ v = immV _ ⌝ ∗
+                                             ↪[frame] _)%I). 
           by iFrame.
           by iIntros "!> [%H _]".
           iIntros (w0) "[-> Hf]".
@@ -3865,33 +5203,23 @@ Definition spec4 idf4 i4 l4 f4 isStack :=
           by destruct Hk2 ; lia.
           iIntros (w0) "(-> & Hs & Himpfcl3 & Hf)".
           iFrame.
-          instantiate (1 := λ v, (⌜ v = immV [value_of_int 4] ⌝ ∗
+          instantiate (1 := λ v, (⌜ v = immV _ ⌝ ∗
                                              isStack k [] ∗
                                              N.of_nat idf3 ↦[wf] FC_func_native i3 (Tf [T_i32] [T_i32]) l3 f3)%I).
           by iFrame.
           iIntros (w0) "[(-> & Hs & Himpfcl3) Hf]".
           iSimpl.
-          instantiate (1:= λ v, (⌜ v = immV [value_of_int 6 ; value_of_int 4] ⌝ ∗
+          instantiate (1:= λ v, (⌜ v = immV _ ⌝ ∗
                                             isStack k [] ∗
                                             N.of_nat idf3 ↦[wf] FC_func_native i3 (Tf [T_i32] [T_i32]) l3 f3 ∗
-                                            ↪[frame] {|
-                                              f_locs := [VAL_int32 (Wasm_int.Int32.repr k)];
-                                              f_inst :=
-                                              {|
-                                                inst_types :=
-                                                [Tf [] []; Tf [] [T_i32]; Tf [T_i32] [T_i32];
-                                                 Tf [T_i32; T_i32] []];
-                                                inst_funcs := [idf0; idf1; idf2; idf3; idf4; idnstart];
-                                                inst_tab := [];
-                                                inst_memory := [];
-                                                inst_globs := [g]
-                                              |}
-                                            |})%I).
+                                            ↪[frame] _)%I ). 
           by iFrame.
           by iIntros "!> [%H _]".
           iIntros (w0) "(-> & Hs & Himpfcl3 & Hf)".
           iSimpl.
-          rewrite (separate3 (i32const _)).
+          rewrite (separate3 (i32const _) (i32const _)).
+          iSimpl.
+          rewrite (separate3 (i32const _) (i32const _)).
           iApply wp_seq.
           iSplitR ; last first.
           iSplitL "Hf".
@@ -3901,15 +5229,17 @@ Definition spec4 idf4 i4 l4 f4 isStack :=
           unfold Wasm_int.Int32.isub, Wasm_int.Int32.sub.
           rewrite Wasm_int.Int32.unsigned_repr.
           rewrite Wasm_int.Int32.unsigned_repr.
-          instantiate (1 := λ v, ⌜ v = immV [value_of_int 2] ⌝%I).
+          instantiate (1 := λ v, ⌜ v = immV _ ⌝%I).
           done.
           unfold Wasm_int.Int32.max_unsigned, Wasm_int.Int32.modulus.
           unfold Wasm_int.Int32.wordsize, Integers.Wordsize_32.wordsize.
           replace (two_power_nat 32) with two32 ; last done.
+          unfold two32.
           lia.
           unfold Wasm_int.Int32.max_unsigned, Wasm_int.Int32.modulus.
           unfold Wasm_int.Int32.wordsize, Integers.Wordsize_32.wordsize.
           replace (two_power_nat 32) with two32 ; last done.
+          unfold two32.
           lia.
           iIntros (w0) "[-> Hf]".
           iSimpl.
@@ -3940,7 +5270,7 @@ Definition spec4 idf4 i4 l4 f4 isStack :=
           done.
           all: try by iIntros "[% _]".
           all: try by iIntros "[[% _] _]".
-          instantiate ( 1 := λ v, (⌜ v = immV [] ⌝ ∗ ∃ g, (N.of_nat g↦[wg] {| g_mut := MUT_mut ; g_val := value_of_int 2 |} ∨ N.of_nat g↦[wg] {| g_mut := MUT_mut ; g_val := value_of_int (-1) |}) ∗ 5%N ↪[vis] {|
+          instantiate ( 1 := λ v, (⌜ v = immV [] ⌝ ∗ ∃ g, (N.of_nat g↦[wg] {| g_mut := MUT_mut ; g_val := value_of_int 20 |} ∨ N.of_nat g↦[wg] {| g_mut := MUT_mut ; g_val := value_of_int (-1) |}) ∗ 7%N ↪[vis] {|
                                                                                                                                                                                                      modexp_name := name;
                            modexp_desc :=
                              MED_global (Mk_globalidx g)
@@ -3983,6 +5313,7 @@ Definition spec4 idf4 i4 l4 f4 isStack :=
                      (BI_const (VAL_int32 (Wasm_int.Int32.repr 6)));
                    AI_basic (BI_get_local 0);
                    AI_basic (BI_call 4);
+                   i32const 0 ; AI_basic (BI_get_local 0) ; AI_basic (BI_call 5) ;                                  
                    AI_basic (BI_get_local 0);
                    AI_basic (BI_call 3);
                    AI_basic (BI_get_local 0);
@@ -4019,10 +5350,10 @@ Definition spec4 idf4 i4 l4 f4 isStack :=
           done. }
       iIntros (w0) "[[-> Hwg] Hf]".
       iFrame.
-      iDestruct "Hwg" as (g') "[Hwg Hvis5]".
+      iDestruct "Hwg" as (g') "[Hwg Hvis7]".
       iExists g', _.
       iFrame.
-  Qed. 
+  Admitted.
 
   End Client.
 End stack.    
